WIP

doc/coq/test.v
@@ -1,5 +1,10 @@
-Require Export Coq.Init.Nat. 
-Require Export Lia.
+From Coq Require Export Bool.Bool.
+From Coq Require Export Init.Nat.
+From Coq Require Export Arith.Arith.
+From Coq Require Export Arith.EqNat.
+From Coq Require Export Lia.
+From Coq Require Export Lists.List.
+From Coq Require Export Strings.String.
 
 Notation "x :: y" := (cons x y)
                      (at level 60, right associativity).
@@ -36,21 +41,6 @@ Inductive value : expr_tm -> Prop :=
 Scheme expr_ind_mut := Induction for expr_tm Sort Prop
 with mod_ind_mut := Induction for mod_tm Sort Prop.
 
-Inductive ctx :=
-  | c_hole
-  | c_lam (x: expr_id) (C : ctx)
-  | c_lete (x : expr_id) (C : ctx)
-  | c_letm (M : mod_id) (C : ctx)
-.
-
-Fixpoint plugin_c Cout Cin :=
-  match Cout with
-  | c_hole => Cin
-  | c_lam x C' => c_lam x (plugin_c C' Cin)
-  | c_lete x C' => c_lete x (plugin_c C' Cin)
-  | c_letm M C' => c_letm M (plugin_c C' Cin)
-  end.
-
 Definition time := nat.
 
 Definition path := list time.
@@ -71,6 +61,21 @@ Fixpoint eq_p (p1 p2 : path) :=
 
 Definition len_p (p : path) := List.length p.
 
+Inductive dy_ctx :=
+  | dy_c_hole
+  | dy_c_lam (x: expr_id) (tx : time) (C : dy_ctx)
+  | dy_c_lete (x : expr_id) (tx : time) (C : dy_ctx)
+  | dy_c_letm (M : mod_id) (CM : dy_ctx) (C : dy_ctx)
+.
+
+Fixpoint dy_plugin_c Cout Cin :=
+  match Cout with
+  | dy_c_hole => Cin
+  | dy_c_lam x tx C' => dy_c_lam x tx (dy_plugin_c C' Cin)
+  | dy_c_lete x tx C' => dy_c_lete x tx (dy_plugin_c C' Cin)
+  | dy_c_letm M CM C' => dy_c_letm M CM (dy_plugin_c C' Cin)
+  end.
+
 Definition eq_eid id1 id2 :=
   match id1, id2 with
   | eid x1, eid x2 => x1 =? x2
@@ -81,168 +86,45 @@ Definition eq_mid id1 id2 :=
   | mid M1, mid M2 => M1 =? M2
   end.
 
-Fixpoint level (C : ctx) :=
+Fixpoint dy_level (C : dy_ctx) : path :=
   match C with
-  | c_hole => 0
-  | c_lam _ C'
-  | c_lete _  C' 
-  | c_letm _  C' => S (level C')
+  | dy_c_hole => []
+  | dy_c_lam _ t C'
+  | dy_c_lete _ t  C' => t :: dy_level C'
+  | dy_c_letm _ _  C' => dy_level C'
   end.
 
-Fixpoint index_expr (C : ctx) (x : expr_id) :=
+Fixpoint addr_x (C : dy_ctx) (x : expr_id) :=
   match C with
-  | c_hole => None
-  | c_lam x' C' 
-  | c_lete x' C' =>
-    match index_expr C' x with
-    | None => if eq_eid x x' then Some (level C') else None
-    | Some i => Some i
+  | dy_c_hole => []
+  | dy_c_lam x' tx' C'
+  | dy_c_lete x' tx' C' =>
+    match addr_x C' x with
+    | [] => if eq_eid x x' then [tx'] else []
+    | addr => tx' :: addr
     end
-  | c_letm _ C' => index_expr C' x
+  | dy_c_letm _ _ C' => addr_x C' x
   end.
 
-Fixpoint index_expr_aux (C : ctx) (x : expr_id) (o : option nat) :=
+Fixpoint ctx_M (C : dy_ctx) (M : mod_id) :=
   match C with
-  | c_hole => o
-  | c_lam x' C' 
-  | c_lete x' C' => 
-    if eq_eid x x' then (
-      index_expr_aux C' x (Some 0)
-    ) else (
-      match o with
-      | Some i => index_expr_aux C' x (Some (S i))
-      | None => index_expr_aux C' x None
-      end
-    )
-  | c_letm _ C' =>
-    match o with
-    | Some i => index_expr_aux C' x (Some (S i))
-    | None => index_expr_aux C' x None
+  | dy_c_hole => None
+  | dy_c_lam _ _ C'
+  | dy_c_lete _ _ C' => ctx_M C' M
+  | dy_c_letm M' CM' C' =>
+    match ctx_M C' M with
+    | Some CM => Some CM
+    | None => if eq_mid M M' then Some CM' else None
     end
   end.
-
-Lemma index_expr_util1 :
-  (forall C x x', index_expr (c_lam x' C) x = None ->
-                  index_expr C x = None) /\
-  (forall C x x', index_expr (c_lete x' C) x = None ->
-                  index_expr C x = None) /\
-  (forall C x M, index_expr (c_letm M C) x = None ->
-                 index_expr C x = None) /\
-  (forall C x m n, index_expr_aux C x None = Some n ->
-                   index_expr_aux C x (Some m) = Some n).
-Proof.
-  repeat split; try (intros; simpl in *; destruct (index_expr C x); eauto; fail);
-                induction C; eauto using ctx; intros; try (inversion H; fail);
-                try (simpl in *; destruct (eq_eid x0 x); eauto; fail).
-Qed.
-
-Lemma index_expr_util2 : forall C n x (NOx : index_expr C x = None),
-                        index_expr_aux C x (Some n) = Some (n + level C).
-Proof.
-  pose proof index_expr_util1 as H; destruct H as [LAM [LETe [LETm IRREL]]].
-  induction C; eauto using ctx;
-  induction n; intros; simpl; eauto; try (
-  try (intros; simpl; fail);
-  remember (eq_eid x0 x) as eid_sub; destruct eid_sub;
-  try (simpl in NOx; rewrite <- Heqeid_sub in NOx;
-  destruct (index_expr C x0); simpl in NOx; inversion NOx; fail));
-  try (replace (S (n + S (level C))) with (S (S n) + level C) by eauto); eauto.
-Qed.
-
-Ltac index_expr_util :=
-  pose proof index_expr_util1 as H; destruct H as [LAM [LETe [LETm IRREL]]];
-  pose proof index_expr_util2 as LEVEL.
-
-Lemma index_expr_eqv_None : forall C x (NOx : index_expr C x = None),
-                        index_expr_aux C x None = None.
-Proof.
-  induction C; eauto using ctx; intros; simpl in NOx;
-  remember (eq_eid x0 x) as eid_sub; destruct eid_sub;
-  try (simpl; destruct (index_expr C x0) in NOx; inversion NOx; fail); 
-  try (
-    remember (index_expr C x0) as i_sub; destruct i_sub; inversion NOx;
-    simpl; rewrite <- Heqeid_sub; apply IHC; eauto; fail).
-Qed.
-
-Lemma index_expr_eqv_Some : forall C x n (SOMEx : index_expr C x = Some n),
-                               index_expr_aux C x None = Some n.
-Proof.
-  index_expr_util. induction C; eauto using ctx; intros.
-  - simpl in SOMEx. remember (index_expr C x0) as i_sub. destruct i_sub.
-    + rewrite SOMEx in *; clear SOMEx.
-      simpl. remember (eq_eid x0 x) as eid_sub. destruct eid_sub;
-      try apply IRREL; apply IHC; eauto.
-    + remember (eq_eid x0 x) as eid_sub. destruct eid_sub.
-      * rewrite <- SOMEx in *. simpl. rewrite <- Heqeid_sub. eauto.
-      * inversion SOMEx.
-  - simpl in SOMEx. remember (index_expr C x0) as i_sub. destruct i_sub.
-    + rewrite SOMEx in *; clear SOMEx.
-      simpl. remember (eq_eid x0 x) as eid_sub. destruct eid_sub;
-      try apply IRREL; apply IHC; eauto.
-    + remember (eq_eid x0 x) as eid_sub. destruct eid_sub.
-      * rewrite <- SOMEx in *. simpl. rewrite <- Heqeid_sub. eauto.
-      * inversion SOMEx.
-Qed.
-
-Theorem index_expr_eqv : forall C x, index_expr C x = index_expr_aux C x None.
-Proof.
-  intros. remember (index_expr C x) as i. destruct i.
-  - symmetry. apply index_expr_eqv_Some; eauto.
-  - symmetry. apply index_expr_eqv_None; eauto.
-Qed.
-
-Fixpoint index_mod (C : ctx) (M : mod_id) :=
-  match C with
-  | c_hole => None
-  | c_lam _ C' 
-  | c_lete _ C' => index_mod C' M
-  | c_letm M' C' => 
-    match index_mod C' M with
-    | None => if eq_mid M M' then Some (level C') else None
-    | Some i => Some i
-    end
-  end.
-
-Fixpoint index_mod_aux (C : ctx) (M : mod_id) (o : option nat) :=
-  match C with
-  | c_hole => o
-  | c_lam _ C'
-  | c_lete _ C' =>
-    match o with
-    | Some i => index_mod_aux C' M (Some (S i))
-    | None => index_mod_aux C' M None
-    end
-  | c_letm M' C' =>
-    if eq_mid M M' then
-      index_mod_aux C' M (Some 0)
-    else match o with
-      | Some i => index_mod_aux C' M (Some (S i))
-      | None => index_mod_aux C' M None
-    end
-  end.
-
-Fixpoint pop (p : path) (i : nat) := 
-  match i with
-  | 0 => Some p
-  | S i' =>
-    match p with
-    | [] => None
-    | _ :: tl => pop tl i'
-    end
-  end.
-
-Inductive mod_value :=
-  | Mod (p : path) (C : ctx)
-.
 
 (* a term, a proof, a path, a context *)
 Inductive expr_value :=
-  | Val (e : expr_tm) (v : value e) (p : path) (C : ctx)
+  | Val (e : expr_tm) (v : value e) (C : dy_ctx)
 .
 
 Inductive state :=
-  | ST (e_mem : path -> option expr_value)
-       (m_mem : path -> option mod_value)
+  | ST (mem : path -> option expr_value)
        (t : time)
 .
 
@@ -254,391 +136,371 @@ Definition empty_mem {X} (p : path) : option X := None.
 Notation "p '!->' v ';' mem" := (update_m mem p v)
                               (at level 100, v at next level, right associativity).
 
-Notation "Cout '[|' Cin '|]'" := (plugin_c Cout Cin)
+Notation "Cout '[|' Cin '|]'" := (dy_plugin_c Cout Cin)
                               (at level 100, Cin at next level, right associativity).
 
-Inductive EevalR (p : path) (C : ctx) (st : state)
+Inductive EevalR (C : dy_ctx) (st : state)
     : expr_tm -> expr_value -> state -> Prop :=
-  | Eeval_var x i p_x v e_mem m_mem t
-             (STATE : ST e_mem m_mem t = st)
-             (INDEX : Some i = index_expr C x)
-             (POP : Some p_x = pop p i)
-             (ACCESS : Some v = e_mem p_x)
-    : EevalR p C st (e_var x) v st
+  | Eeval_var x v mem t
+             (STATE : ST mem t = st)
+             (ADDR : [] <> addr_x C x)
+             (ACCESS : Some v = mem (addr_x C x))
+    : EevalR C st (e_var x) v st
   | Eeval_lam x e
-    : EevalR p C st (e_lam x e) 
-            (Val (e_lam x e) (v_fn x e) p C) st
+    : EevalR C st (e_lam x e)
+            (Val (e_lam x e) (v_fn x e) C) st
   | Eeval_app e1 e2 
-              x e p_lam C_lam st_lam
-              arg e_mem m_mem t
+              x e C_lam st_lam
+              arg mem t
               v st_v
-              (FN : EevalR p C st e1
-                           (Val (e_lam x e) (v_fn x e) p_lam C_lam) st_lam)
-              (ARG : EevalR p C st_lam e2
-                            arg (ST e_mem m_mem t))
-              (BODY : EevalR (t :: p_lam) (C_lam [|c_lam x c_hole|])
-                             (ST ((t :: p_lam) !-> arg ; e_mem) m_mem (update_t t))
+              (FN : EevalR C st e1
+                           (Val (e_lam x e) (v_fn x e) C_lam) st_lam)
+              (ARG : EevalR C st_lam e2
+                            arg (ST mem t))
+              (BODY : EevalR (C_lam [|dy_c_lam x t dy_c_hole|])
+                             (ST ((dy_level C_lam) ++ [t] !-> arg ; mem) (update_t t))
                               e v st_v)
-    : EevalR p C st (e_app e1 e2) v st_v
-  | Eeval_link m e p_m C_m st_m v st_v
-               (MOD : MevalR p C st m (Mod p_m C_m) st_m)
-               (LINK : EevalR p_m C_m st_m e v st_v)
-    : EevalR p C st (e_link m e) v st_v
+    : EevalR C st (e_app e1 e2) v st_v
+  | Eeval_link m e C_m st_m v st_v
+               (MOD : MevalR C st m C_m st_m)
+               (LINK : EevalR C_m st_m e v st_v)
+    : EevalR C st (e_link m e) v st_v
 
-with MevalR (p : path) (C : ctx) (st : state)
-    : mod_tm -> mod_value -> state -> Prop :=
+with MevalR (C : dy_ctx) (st : state)
+    : mod_tm -> dy_ctx -> state -> Prop :=
   | Meval_empty
-    : MevalR p C st m_empty (Mod p C) st
-  | Meval_var M i p_M v e_mem m_mem t
-              (STATE : ST e_mem m_mem t = st)
-              (INDEX : Some i = index_mod C M)
-              (POP : Some p_M = pop p i)
-              (ACCESS : Some v = m_mem p_M)
-    : MevalR p C st (m_var M) v st
-  | Meval_lete x e v_e e_mem m_mem t
-               m v_m st_m
-               (EVALe : EevalR p C st e v_e (ST e_mem m_mem t))
-               (EVALm : MevalR (t :: p) (C [|c_lete x c_hole|]) 
-                        (ST ((t :: p) !-> v_e ; e_mem) m_mem (update_t t))
-                        m v_m st_m)
-    : MevalR p C st (m_lete x e m) v_m st_m
-  | Meval_letm M m1 v_m1 e_mem m_mem t
-               m2 v_m2 st_m2
-               (EVALm1 : MevalR p C st m1 v_m1 (ST e_mem m_mem t))
-               (EVALm2 : MevalR (t :: p) (C [|c_letm M c_hole|])
-                         (ST e_mem ((t :: p) !-> v_m1 ; m_mem) (update_t t))
-                         m2 v_m2 st_m2)
-    : MevalR p C st (m_letm M m1 m2) v_m2 st_m2
+    : MevalR C st m_empty C st
+  | Meval_var M C_M (ACCESS : Some C_M = ctx_M C M)
+    : MevalR C st (m_var M) C_M st
+  | Meval_lete x e v_e mem t
+               m C_m st_m
+               (EVALe : EevalR C st e v_e (ST mem t))
+               (EVALm : MevalR (C [|dy_c_lete x t dy_c_hole|]) 
+                        (ST ((dy_level C ++ [t]) !-> v_e ; mem) (update_t t))
+                        m C_m st_m)
+    : MevalR C st (m_lete x e m) C_m st_m
+  | Meval_letm M m1 C_m1 st_m1
+               m2 C_m2 st_m2
+               (EVALm1 : MevalR C st m1 C_m1 st_m1)
+               (EVALm2 : MevalR (C [|dy_c_letm M C_m1 dy_c_hole|]) st_m1
+                         m2 C_m2 st_m2)
+    : MevalR C st (m_letm M m1 m2) C_m2 st_m2
 .
 
 Scheme EevalR_ind_mut := Induction for EevalR Sort Prop
 with MevalR_ind_mut := Induction for MevalR Sort Prop.
 
-Definition Reach (tm1 tm2 : Type) := tm1 -> path -> ctx -> state -> tm2 -> Prop.
+Definition Reach (tm1 tm2 : Type) := tm1 -> dy_ctx -> state -> tm2 -> Prop.
 
 (* Reachability relation, sensible version *)
-Inductive _EreachE (p : path) (C : ctx) (st : state)
+Inductive _EreachE (C : dy_ctx) (st : state)
     : Reach expr_tm expr_tm :=
   | _ere_refl e
-    : _EreachE p C st e 
-               p C st e
-  | _ere_var x i p_x e_mem m_mem t v pf p_v C_v
-            (STATE : ST e_mem m_mem t = st)
-            (INDEX : Some i = index_expr C x)
-            (POP : Some p_x = pop p i)
-            (ACCESS : Some (Val v pf p_v C_v) = e_mem p_x)
-    : _EreachE p C st (e_var x) 
-               p_v C_v st v
-  | _ere_app_left e1 e2 p' C' st' e'
-                 (REACHl : _EreachE p C st e1
-                                    p' C' st' e')
-    : _EreachE p C st (e_app e1 e2) 
-               p' C' st' e'
-  | _ere_app_right e1 e2 st1 v p' C' st' e'
-                  (FN : EevalR p C st e1 v st1)
-                  (REACHr : _EreachE p C st1 e2
-                                     p' C' st' e')
-    : _EreachE p C st (e_app e1 e2)
-               p' C' st' e'
-  | _ere_app_body e1 e2 x e p_lam C_lam st_lam
-                 arg e_mem m_mem t
-                 p' C' st' e'
-                 (FN : EevalR p C st e1 
-                             (Val (e_lam x e) (v_fn x e) p_lam C_lam) st_lam)
-                 (ARG : EevalR p C st_lam e2
-                               arg (ST e_mem m_mem t))
-                 (REACHb : _EreachE (t :: p_lam) (C_lam[|c_lam x c_hole|]) 
-                                    (ST ((t :: p_lam) !-> arg ; e_mem) m_mem (update_t t)) e
-                                     p' C' st' e')
-    : _EreachE p C st (e_app e1 e2)
-               p' C' st' e'
-  | _ere_link_m m e p' C' st' e'
-               (REACHm : _MreachE p C st m
-                                  p' C' st' e')
-    : _EreachE p C st (e_link m e)
-               p' C' st' e'
-  | _ere_link_e m e p_m C_m st_m p' C' st' e'
-               (MOD : MevalR p C st m (Mod p_m C_m) st_m)
-               (REACHe : _EreachE p_m C_m st_m e
-                                  p' C' st' e')
-    : _EreachE p C st (e_link m e)
-               p' C' st' e'
+    : _EreachE C st e 
+               C st e
+  | _ere_var x mem t v pf C_v
+            (STATE : ST mem t = st)
+            (ADDR : [] <> addr_x C x)
+            (ACCESS : Some (Val v pf C_v) = mem (addr_x C x))
+    : _EreachE C st (e_var x) 
+               C_v st v
+  | _ere_app_left e1 e2 C' st' e'
+                 (REACHl : _EreachE C st e1
+                                    C' st' e')
+    : _EreachE C st (e_app e1 e2) 
+               C' st' e'
+  | _ere_app_right e1 e2 st1 v C' st' e'
+                  (FN : EevalR C st e1 v st1)
+                  (REACHr : _EreachE C st1 e2
+                                     C' st' e')
+    : _EreachE C st (e_app e1 e2)
+               C' st' e'
+  | _ere_app_body e1 e2 x e C_lam st_lam
+                 arg mem t
+                 C' st' e'
+                 (FN : EevalR C st e1 
+                             (Val (e_lam x e) (v_fn x e) C_lam) st_lam)
+                 (ARG : EevalR C st_lam e2
+                               arg (ST mem t))
+                 (REACHb : _EreachE (C_lam[|dy_c_lam x t dy_c_hole|]) 
+                                    (ST ((dy_level C_lam ++ [t]) !-> arg ; mem) (update_t t)) e
+                                     C' st' e')
+    : _EreachE C st (e_app e1 e2)
+               C' st' e'
+  | _ere_link_m m e C' st' e'
+               (REACHm : _MreachE C st m
+                                  C' st' e')
+    : _EreachE C st (e_link m e)
+               C' st' e'
+  | _ere_link_e m e C_m st_m C' st' e'
+               (MOD : MevalR C st m C_m st_m)
+               (REACHe : _EreachE C_m st_m e
+                                  C' st' e')
+    : _EreachE C st (e_link m e)
+               C' st' e'
 
-with _MreachE (p : path) (C : ctx) (st : state)
+with _MreachE (C : dy_ctx) (st : state)
     : Reach mod_tm expr_tm :=
-  | _mre_lete_e x e m p' C' st' e'
-               (REACHe : _EreachE p C st e
-                                  p' C' st' e')
-    : _MreachE p C st (m_lete x e m)
-               p' C' st' e'
-  | _mre_lete_m x e m v e_mem m_mem t
-             p' C' st' e'
-             (EVALx : EevalR p C st e v (ST e_mem m_mem t))
-             (REACHm : _MreachE (t :: p) (C[|c_lete x c_hole|])
-                                (ST ((t :: p) !-> v ; e_mem) m_mem (update_t t)) m
-                                 p' C' st' e')
-    : _MreachE p C st (m_lete x e m)
-               p' C' st' e'
-  | _mre_letm_m1 M m1 m2 p' C' st' e'
-               (REACHm : _MreachE p C st m1
-                                  p' C' st' e')
-    : _MreachE p C st (m_letm M m1 m2)
-              p' C' st' e'
-  | _mre_letm_m2 M m1 m2 v e_mem m_mem t
-             p' C' st' e'
-             (EVALM : MevalR p C st m1 v (ST e_mem m_mem t))
-             (REACHm : _MreachE (t :: p) (C[|c_letm M c_hole|]) 
-                                (ST e_mem ((t :: p) !-> v ; m_mem) (update_t t)) m2
-                                 p' C' st' e')
-    : _MreachE p C st (m_letm M m1 m2)
-               p' C' st' e'.
+  | _mre_lete_e x e m C' st' e'
+               (REACHe : _EreachE C st e
+                                  C' st' e')
+    : _MreachE C st (m_lete x e m)
+               C' st' e'
+  | _mre_lete_m x e m v mem t
+                C' st' e'
+             (EVALx : EevalR C st e v (ST mem t))
+             (REACHm : _MreachE (C[|dy_c_lete x t dy_c_hole|])
+                                (ST ((dy_level C ++ [t]) !-> v ; mem) (update_t t)) m
+                                 C' st' e')
+    : _MreachE C st (m_lete x e m)
+               C' st' e'
+  | _mre_letm_m1 M m1 m2 C' st' e'
+               (REACHm : _MreachE C st m1
+                                  C' st' e')
+    : _MreachE C st (m_letm M m1 m2)
+               C' st' e'
+  | _mre_letm_m2 M m1 m2 C_M st_M
+                 C' st' e'
+             (EVALM : MevalR C st m1 C_M st_M)
+             (REACHm : _MreachE (C[|dy_c_letm M C_M dy_c_hole|]) st_M m2
+                                 C' st' e')
+    : _MreachE C st (m_letm M m1 m2)
+               C' st' e'.
 
 Scheme __EreachE_ind_mut := Induction for _EreachE Sort Prop
 with __MreachE_ind_mut := Induction for _MreachE Sort Prop.
 
-Inductive _MreachM (p : path) (C : ctx) (st : state)
+Inductive _MreachM (C : dy_ctx) (st : state)
     : Reach mod_tm mod_tm :=
   | _mrm_refl m
-    : _MreachM p C st m
-               p C st m
-  | _mrm_var M i p_M e_mem m_mem t p_v C_v
-            (STATE : ST e_mem m_mem t = st)
-            (INDEX : Some i = index_mod C M)
-            (POP : Some p_M = pop p i)
-            (ACCESS : Some (Mod p_v C_v) = m_mem p_M)
-    : _MreachM p C st (m_var M)
-               p_v C_v st m_empty
-  | _mrm_lete_e x e m p' C' st' m'
-               (REACHe : _EreachM p C st e
-                                  p' C' st' m')
-    : _MreachM p C st (m_lete x e m)
-               p' C' st' m'
-  | _mrm_lete_m x e m v e_mem m_mem t
-             p' C' st' m'
-             (EVALx : EevalR p C st e v (ST e_mem m_mem t))
-             (REACHm : _MreachM (t :: p) (C[|c_lete x c_hole|]) 
-                                (ST ((t :: p) !-> v ; e_mem) m_mem (update_t t)) m
-                                 p' C' st' m')
-    : _MreachM p C st (m_lete x e m)
-               p' C' st' m'
-  | _mrm_letm_m1 M m1 m2 p' C' st' m'
-               (REACHm : _MreachM p C st m1
-                                  p' C' st' m')
-    : _MreachM p C st (m_letm M m1 m2)
-               p' C' st' m'
-  | _mrm_letm_m2 M m1 m2 v e_mem m_mem t
-             p' C' st' m'
-             (EVALM : MevalR p C st m1 v (ST e_mem m_mem t))
-             (REACHm : _MreachM (t :: p) (C[|c_letm M c_hole|]) 
-                                (ST e_mem ((t :: p) !-> v ; m_mem) (update_t t)) m2
-                                 p' C' st' m')
-    : _MreachM p C st (m_letm M m1 m2)
-               p' C' st' m'
+    : _MreachM C st m
+               C st m
+  | _mrm_var M C_M (ACCESS : Some C_M = ctx_M C M)
+    : _MreachM C st (m_var M)
+               C_M st m_empty
+  | _mrm_lete_e x e m C' st' m'
+               (REACHe : _EreachM C st e
+                                  C' st' m')
+    : _MreachM C st (m_lete x e m)
+               C' st' m'
+  | _mrm_lete_m x e m v mem t
+                C' st' m'
+             (EVALx : EevalR C st e v (ST mem t))
+             (REACHm : _MreachM (C[|dy_c_lete x t dy_c_hole|]) 
+                                (ST ((dy_level C ++ [t]) !-> v ; mem) (update_t t)) m
+                                 C' st' m')
+    : _MreachM C st (m_lete x e m)
+               C' st' m'
+  | _mrm_letm_m1 M m1 m2 C' st' m'
+               (REACHm : _MreachM C st m1
+                                  C' st' m')
+    : _MreachM C st (m_letm M m1 m2)
+               C' st' m'
+  | _mrm_letm_m2 M m1 m2 C_M st_M
+                 C' st' m'
+             (EVALM : MevalR C st m1 C_M st_M)
+             (REACHm : _MreachM (C[|dy_c_letm M C_M dy_c_hole|]) st_M m2
+                                 C' st' m')
+    : _MreachM C st (m_letm M m1 m2)
+               C' st' m'
 
-with _EreachM (p : path) (C : ctx) (st : state)
+with _EreachM (C : dy_ctx) (st : state)
     : Reach expr_tm mod_tm :=
-  | _erm_app_left e1 e2 p' C' st' m'
-                 (REACHl : _EreachM p C st e1
-                                    p' C' st' m')
-    : _EreachM p C st (e_app e1 e2) 
-               p' C' st' m'
-  | _erm_app_right e1 e2 v1 st1 p' C' st' m'
-                  (FN : EevalR p C st e1 v1 st1)
-                  (REACHr : _EreachM p C st1 e2
-                                     p' C' st' m')
-    : _EreachM p C st (e_app e1 e2)
-               p' C' st' m'
-  | _erm_app_body e1 e2 x e p_lam C_lam st_lam
-                 arg e_mem m_mem t
-                 p' C' st' m'
-                 (FN : EevalR p C st e1 
-                              (Val (e_lam x e) (v_fn x e) p_lam C_lam) st_lam)
-                 (ARG : EevalR p C st_lam e2 arg (ST e_mem m_mem t))
-                 (REACHb : _EreachM (t :: p_lam) (C_lam[|c_lam x c_hole|]) 
-                                    (ST ((t :: p_lam) !-> arg ; e_mem) m_mem (update_t t)) e
-                                     p' C' st' m')
-    : _EreachM p C st (e_app e1 e2)
-               p' C' st' m'
-  | _erm_link_m m e p' C' st' m'
-               (REACHm : _MreachM p C st m
-                                  p' C' st' m')
-    : _EreachM p C st (e_link m e)
-               p' C' st' m'
-  | _erm_link_e m e p_m C_m st_m p' C' st' m'
-               (MOD : MevalR p C st m (Mod p_m C_m) st_m)
-               (REACHe : _EreachM p_m C_m st_m e
-                                  p' C' st' m')
-    : _EreachM p C st (e_link m e)
-               p' C' st' m'
+  | _erm_app_left e1 e2 C' st' m'
+                 (REACHl : _EreachM C st e1
+                                    C' st' m')
+    : _EreachM C st (e_app e1 e2) 
+               C' st' m'
+  | _erm_app_right e1 e2 v1 st1 C' st' m'
+                  (FN : EevalR C st e1 v1 st1)
+                  (REACHr : _EreachM C st1 e2
+                                     C' st' m')
+    : _EreachM C st (e_app e1 e2)
+               C' st' m'
+  | _erm_app_body e1 e2 x e C_lam st_lam
+                 arg mem t
+                 C' st' m'
+                 (FN : EevalR C st e1 
+                              (Val (e_lam x e) (v_fn x e) C_lam) st_lam)
+                 (ARG : EevalR C st_lam e2 arg (ST mem t))
+                 (REACHb : _EreachM (C_lam[|dy_c_lam x t dy_c_hole|]) 
+                                    (ST ((dy_level C_lam ++ [t]) !-> arg ; mem) (update_t t)) e
+                                     C' st' m')
+    : _EreachM C st (e_app e1 e2)
+               C' st' m'
+  | _erm_link_m m e C' st' m'
+               (REACHm : _MreachM C st m
+                                  C' st' m')
+    : _EreachM C st (e_link m e)
+               C' st' m'
+  | _erm_link_e m e C_m st_m C' st' m'
+               (MOD : MevalR C st m C_m st_m)
+               (REACHe : _EreachM C_m st_m e
+                                  C' st' m')
+    : _EreachM C st (e_link m e)
+               C' st' m'
 .
 
 Scheme __EreachM_ind_mut := Induction for _EreachM Sort Prop
 with __MreachM_ind_mut := Induction for _MreachM Sort Prop.
 
 (* for proofs *)
-Inductive EreachE (p : path) (C : ctx) (st : state)
+Inductive EreachE (C : dy_ctx) (st : state)
     : Reach expr_tm expr_tm :=
   | ere_refl e
-    : EreachE p C st e 
-              p C st e
-  | ere_var x i p_x e_mem m_mem t v pf p_v C_v
-            (STATE : ST e_mem m_mem t = st)
-            (INDEX : Some i = index_expr C x)
-            (POP : Some p_x = pop p i)
-            (ACCESS : Some (Val v pf p_v C_v) = e_mem p_x)
-    : EreachE p C st (e_var x) 
-              p_v C_v st v
-  | ere_app_left e1 e2 p' C' st' e'
-                 (REACHl : EreachE p C st e1
-                                   p' C' st' e')
-    : EreachE p C st (e_app e1 e2) 
-              p' C' st' e'
-  | ere_app_right e1 e2 st1 v pf p1 C1 p' C' st' e'
-                  (FN : EevalR p C st e1 (Val v pf p1 C1) st1)
-                  (FNr : EreachE p C st e1 p1 C1 st1 v)
-                  (REACHr : EreachE p C st1 e2
-                                    p' C' st' e')
-    : EreachE p C st (e_app e1 e2)
-              p' C' st' e'
-  | ere_app_body e1 e2 x e p_lam C_lam st_lam
-                 arg pf p_arg C_arg e_mem m_mem t
-                 p' C' st' e'
-                 (FN : EevalR p C st e1 
-                             (Val (e_lam x e) (v_fn x e) p_lam C_lam) st_lam)
-                 (FNr : EreachE p C st e1 p_lam C_lam st_lam (e_lam x e))
-                 (ARG : EevalR p C st_lam e2
-                               (Val arg pf p_arg C_arg) (ST e_mem m_mem t))
-                 (ARGr : EreachE p C st_lam e2 p_arg C_arg (ST e_mem m_mem t) arg)
-                 (REACHb : EreachE (t :: p_lam) (C_lam[|c_lam x c_hole|]) 
-                                   (ST ((t :: p_lam) !-> (Val arg pf p_arg C_arg) ; e_mem) m_mem (update_t t)) e
-                                    p' C' st' e')
-    : EreachE p C st (e_app e1 e2)
-              p' C' st' e'
-  | ere_link_m m e p' C' st' e'
-               (REACHm : MreachE p C st m
-                                 p' C' st' e')
-    : EreachE p C st (e_link m e)
-              p' C' st' e'
-  | ere_link_e m e p_m C_m st_m p' C' st' e'
-               (MOD : MevalR p C st m (Mod p_m C_m) st_m)
-               (MODr : MreachM p C st m p_m C_m st_m m_empty)
-               (REACHe : EreachE p_m C_m st_m e
-                                 p' C' st' e')
-    : EreachE p C st (e_link m e)
-              p' C' st' e'
+    : EreachE C st e 
+               C st e
+  | ere_var x mem t v pf C_v
+            (STATE : ST mem t = st)
+            (ADDR : [] <> addr_x C x)
+            (ACCESS : Some (Val v pf C_v) = mem (addr_x C x))
+    : EreachE C st (e_var x) 
+               C_v st v
+  | ere_app_left e1 e2 C' st' e'
+                 (REACHl : EreachE C st e1
+                                   C' st' e')
+    : EreachE C st (e_app e1 e2) 
+               C' st' e'
+  | ere_app_right e1 e2 st_lam v pf C_lam C' st' e'
+                  (FN : EevalR C st e1 (Val v pf C_lam) st_lam)
+                  (FNr : EreachE C st e1 C_lam st_lam v)
+                  (REACHr : EreachE C st_lam e2
+                                    C' st' e')
+    : EreachE C st (e_app e1 e2)
+              C' st' e'
+  | ere_app_body e1 e2 x e C_lam st_lam
+                 arg pf C_arg mem t
+                 C' st' e'
+                 (FN : EevalR C st e1 
+                             (Val (e_lam x e) (v_fn x e) C_lam) st_lam)
+                 (FNr : EreachE C st e1 C_lam st_lam (e_lam x e))
+                 (ARG : EevalR C st_lam e2
+                               (Val arg pf C_arg) (ST mem t))
+                 (ARGr : EreachE C st_lam e2 C_arg (ST mem t) arg)
+                 (REACHb : EreachE (C_lam[|dy_c_lam x t dy_c_hole|]) 
+                                    (ST ((dy_level C_lam ++ [t]) !-> (Val arg pf C_arg) ; mem) (update_t t)) e
+                                     C' st' e')
+    : EreachE C st (e_app e1 e2)
+              C' st' e'
+  | ere_link_m m e C' st' e'
+               (REACHm : MreachE C st m
+                                 C' st' e')
+    : EreachE C st (e_link m e)
+              C' st' e'
+  | ere_link_e m e C_m st_m C' st' e'
+              (MOD : MevalR C st m C_m st_m)
+              (MODr : MreachM C st m C_m st_m m_empty)
+              (REACHe : EreachE C_m st_m e
+                                C' st' e')
+    : EreachE C st (e_link m e)
+              C' st' e'
 
-with MreachE (p : path) (C : ctx) (st : state)
+with MreachE (C : dy_ctx) (st : state)
     : Reach mod_tm expr_tm :=
-  | mre_lete_e x e m p' C' st' e'
-               (REACHe : EreachE p C st e
-                                 p' C' st' e')
-    : MreachE p C st (m_lete x e m)
-              p' C' st' e'
-  | mre_lete_m x e m v pf p1 C1 e_mem m_mem t
-             p' C' st' e'
-             (EVALx : EevalR p C st e (Val v pf p1 C1) (ST e_mem m_mem t))
-             (EVALxr : EreachE p C st e p1 C1 (ST e_mem m_mem t) v)
-             (REACHm : MreachE (t :: p) (C[|c_lete x c_hole|])
-                               (ST ((t :: p) !-> (Val v pf p1 C1) ; e_mem) m_mem (update_t t)) m
-                                p' C' st' e')
-    : MreachE p C st (m_lete x e m)
-              p' C' st' e'
-  | mre_letm_m1 M m1 m2 p' C' st' e'
-               (REACHm : MreachE p C st m1
-                                 p' C' st' e')
-    : MreachE p C st (m_letm M m1 m2)
-              p' C' st' e'
-  | mre_letm_m2 M m1 m2 p_m C_m e_mem m_mem t
-             p' C' st' e'
-             (EVALM : MevalR p C st m1 (Mod p_m C_m) (ST e_mem m_mem t))
-             (EVALMr : MreachM p C st m1 p_m C_m (ST e_mem m_mem t) m_empty)
-             (REACHm : MreachE (t :: p) (C[|c_letm M c_hole|]) 
-                               (ST e_mem ((t :: p) !-> (Mod p_m C_m) ; m_mem) (update_t t)) m2
-                                p' C' st' e')
-    : MreachE p C st (m_letm M m1 m2)
-              p' C' st' e'
+  | mre_lete_e x e m C' st' e'
+               (REACHe : EreachE C st e
+                                 C' st' e')
+    : MreachE C st (m_lete x e m)
+              C' st' e'
+  | mre_lete_m x e m v pf C_x mem t
+               C' st' e'
+             (EVALx : EevalR C st e (Val v pf C_x) (ST mem t))
+             (EVALxr : EreachE C st e C_x (ST mem t) v)
+             (REACHm : MreachE (C[|dy_c_lete x t dy_c_hole|])
+                                (ST ((dy_level C ++ [t]) !-> (Val v pf C_x) ; mem) (update_t t)) m
+                                 C' st' e')
+    : MreachE C st (m_lete x e m)
+              C' st' e'
+  | mre_letm_m1 M m1 m2 C' st' e'
+              (REACHm : MreachE C st m1
+                                C' st' e')
+    : MreachE C st (m_letm M m1 m2)
+              C' st' e'
+  | mre_letm_m2 M m1 m2 C_M st_M
+                C' st' e'
+             (EVALM : MevalR C st m1 C_M st_M)
+             (EVALM : MreachM C st m1 C_M st_M m_empty)
+             (REACHm : MreachE (C[|dy_c_letm M C_M dy_c_hole|]) st_M m2
+                                C' st' e')
+    : MreachE C st (m_letm M m1 m2)
+              C' st' e'
 
-with MreachM (p : path) (C : ctx) (st : state)
+with MreachM (C : dy_ctx) (st : state)
     : Reach mod_tm mod_tm :=
   | mrm_refl m
-    : MreachM p C st m
-              p C st m
-  | mrm_var M i p_M e_mem m_mem t p_v C_v
-            (STATE : ST e_mem m_mem t = st)
-            (INDEX : Some i = index_mod C M)
-            (POP : Some p_M = pop p i)
-            (ACCESS : Some (Mod p_v C_v) = m_mem p_M)
-    : MreachM p C st (m_var M)
-              p_v C_v st m_empty
-  | mrm_lete_e x e m p' C' st' m'
-               (REACHe : EreachM p C st e
-                                 p' C' st' m')
-    : MreachM p C st (m_lete x e m)
-              p' C' st' m'
-  | mrm_lete_m x e m v pf p1 C1 e_mem m_mem t
-             p' C' st' m'
-             (EVALx : EevalR p C st e (Val v pf p1 C1) (ST e_mem m_mem t))
-             (EVALxr : EreachE p C st e p1 C1 (ST e_mem m_mem t) v)
-             (REACHm : MreachM (t :: p) (C[|c_lete x c_hole|])
-                               (ST ((t :: p) !-> (Val v pf p1 C1) ; e_mem) m_mem (update_t t)) m
-                                p' C' st' m')
-    : MreachM p C st (m_lete x e m)
-              p' C' st' m'
-  | mrm_letm_m1 M m1 m2 p' C' st' m'
-               (REACHm : MreachM p C st m1
-                                 p' C' st' m')
-    : MreachM p C st (m_letm M m1 m2)
-              p' C' st' m'
-  | mrm_letm_m2 M m1 m2 p_m C_m e_mem m_mem t
-             p' C' st' m'
-             (EVALM : MevalR p C st m1 (Mod p_m C_m) (ST e_mem m_mem t))
-             (EVALMr : MreachM p C st m1 p_m C_m (ST e_mem m_mem t) m_empty)
-             (REACHm : MreachM (t :: p) (C[|c_letm M c_hole|]) 
-                               (ST e_mem ((t :: p) !-> (Mod p_m C_m) ; m_mem) (update_t t)) m2
-                                p' C' st' m')
-    : MreachM p C st (m_letm M m1 m2)
-              p' C' st' m'
+    : MreachM C st m
+              C st m
+  | mrm_var M C_M (ACCESS : Some C_M = ctx_M C M)
+    : MreachM C st (m_var M)
+              C_M st m_empty
+  | mrm_lete_e x e m C' st' m'
+               (REACHe : EreachM C st e
+                                  C' st' m')
+    : MreachM C st (m_lete x e m)
+              C' st' m'
+  | mrm_lete_m x e m v pf C_x mem t
+               C' st' m'
+             (EVALx : EevalR C st e (Val v pf C_x) (ST mem t))
+             (EVALxr : EreachE C st e C_x (ST mem t) v)
+             (REACHm : MreachM (C[|dy_c_lete x t dy_c_hole|]) 
+                               (ST ((dy_level C ++ [t]) !-> (Val v pf C_x) ; mem) (update_t t)) m
+                                C' st' m')
+    : MreachM C st (m_lete x e m)
+              C' st' m'
+  | mrm_letm_m1 M m1 m2 C' st' m'
+               (REACHm : MreachM C st m1
+                                 C' st' m')
+    : MreachM C st (m_letm M m1 m2)
+              C' st' m'
+  | mrm_letm_m2 M m1 m2 C_M st_M
+                C' st' m'
+             (EVALM : MevalR C st m1 C_M st_M)
+             (EVALMr : MreachM C st m1 C_M st_M m_empty)
+             (REACHm : MreachM (C[|dy_c_letm M C_M dy_c_hole|]) st_M m2
+                                C' st' m')
+    : MreachM C st (m_letm M m1 m2)
+              C' st' m'
 
-with EreachM (p : path) (C : ctx) (st : state)
+with EreachM (C : dy_ctx) (st : state)
     : Reach expr_tm mod_tm :=
-  | erm_app_left e1 e2 p' C' st' m'
-                 (REACHl : EreachM p C st e1
-                                   p' C' st' m')
-    : EreachM p C st (e_app e1 e2) 
-              p' C' st' m'
-  | erm_app_right e1 e2 st1 v pf p1 C1 p' C' st' m'
-                  (FN : EevalR p C st e1 (Val v pf p1 C1) st1)
-                  (FNr : EreachE p C st e1 p1 C1 st1 v)
-                  (REACHr : EreachM p C st1 e2
-                                    p' C' st' m')
-    : EreachM p C st (e_app e1 e2)
-              p' C' st' m'
-  | erm_app_body e1 e2 x e p_lam C_lam st_lam
-                 arg pf p_arg C_arg e_mem m_mem t
-                 p' C' st' m'
-                 (FN : EevalR p C st e1 
-                             (Val (e_lam x e) (v_fn x e) p_lam C_lam) st_lam)
-                 (FNr : EreachE p C st e1 p_lam C_lam st_lam (e_lam x e))
-                 (ARG : EevalR p C st_lam e2
-                               (Val arg pf p_arg C_arg) (ST e_mem m_mem t))
-                 (ARGr : EreachE p C st_lam e2 p_arg C_arg (ST e_mem m_mem t) arg)
-                 (REACHb : EreachM (t :: p_lam) (C_lam[|c_lam x c_hole|]) 
-                                   (ST ((t :: p_lam) !-> (Val arg pf p_arg C_arg) ; e_mem) m_mem (update_t t)) e
-                                    p' C' st' m')
-    : EreachM p C st (e_app e1 e2)
-              p' C' st' m'
-  | erm_link_m m e p' C' st' m'
-               (REACHm : MreachM p C st m
-                                 p' C' st' m')
-    : EreachM p C st (e_link m e)
-              p' C' st' m'
-  | erm_link_e m e p_m C_m st_m p' C' st' m'
-               (MOD : MevalR p C st m (Mod p_m C_m) st_m)
-               (MODr : MreachM p C st m p_m C_m st_m m_empty)
-               (REACHe : EreachM p_m C_m st_m e
-                                 p' C' st' m')
-    : EreachM p C st (e_link m e)
-              p' C' st' m'
+  | erm_app_left e1 e2 C' st' m'
+                (REACHl : EreachM C st e1
+                                  C' st' m')
+    : EreachM C st (e_app e1 e2) 
+              C' st' m'
+  | erm_app_right e1 e2 v pf C_lam st_lam C' st' m'
+                 (FN : EevalR C st e1 (Val v pf C_lam) st_lam)
+                 (FNr : EreachE C st e1 C_lam st_lam v)
+                 (REACHr : EreachM C st_lam e2
+                                   C' st' m')
+    : EreachM C st (e_app e1 e2)
+              C' st' m'
+  | erm_app_body e1 e2 x e C_lam st_lam
+                 arg pf C_arg mem t
+                 C' st' m'
+                 (FN : EevalR C st e1 
+                              (Val (e_lam x e) (v_fn x e) C_lam) st_lam)
+                 (FNr : EreachE C st e1 
+                                C_lam st_lam (e_lam x e))
+                 (ARG : EevalR C st_lam e2 (Val arg pf C_arg) (ST mem t))
+                 (ARGr : EreachE C st_lam e2 C_arg (ST mem t) arg)
+                 (REACHb : EreachM (C_lam[|dy_c_lam x t dy_c_hole|]) 
+                                   (ST ((dy_level C_lam ++ [t]) !-> (Val arg pf C_arg) ; mem) (update_t t)) e
+                                    C' st' m')
+    : EreachM C st (e_app e1 e2)
+              C' st' m'
+  | erm_link_m m e C' st' m'
+              (REACHm : MreachM C st m
+                                C' st' m')
+    : EreachM C st (e_link m e)
+              C' st' m'
+  | erm_link_e m e C_m st_m C' st' m'
+              (MOD : MevalR C st m C_m st_m)
+              (MODr : MreachM C st m C_m st_m m_empty)
+              (REACHe : EreachM C_m st_m e
+                                C' st' m')
+    : EreachM C st (e_link m e)
+              C' st' m'
 .
 
 Scheme _EreachE_ind_mut := Induction for EreachE Sort Prop
@@ -646,178 +508,178 @@ with _EreachM_ind_mut := Induction for EreachM Sort Prop
 with _MreachE_ind_mut := Induction for MreachE Sort Prop
 with _MreachM_ind_mut := Induction for MreachM Sort Prop.
 
-Notation "'<e|' p1 C1 st1 tm1 '~>' p2 C2 st2 tm2 '|e>'" := (EreachE p1 C1 st1 tm1 p2 C2 st2 tm2) 
+Notation "'<e|' C1 st1 tm1 '~>' C2 st2 tm2 '|e>'" := (EreachE C1 st1 tm1 C2 st2 tm2) 
                                                (at level 10, 
-                                                p1 at next level, C1 at next level, st1 at next level, tm1 at next level,
-                                                p2 at next level, C2 at next level, st2 at next level, tm2 at next level).
+                                                C1 at next level, st1 at next level, tm1 at next level,
+                                                C2 at next level, st2 at next level, tm2 at next level).
 
-Notation "'<m|' p1 C1 st1 tm1 '~>' p2 C2 st2 tm2 '|e>'" := (MreachE p1 C1 st1 tm1 p2 C2 st2 tm2) 
+Notation "'<m|' C1 st1 tm1 '~>' C2 st2 tm2 '|e>'" := (MreachE C1 st1 tm1 C2 st2 tm2) 
                                                (at level 10, 
-                                                p1 at next level, C1 at next level, st1 at next level, tm1 at next level,
-                                                p2 at next level, C2 at next level, st2 at next level, tm2 at next level).
+                                                C1 at next level, st1 at next level, tm1 at next level,
+                                                C2 at next level, st2 at next level, tm2 at next level).
 
-Notation "'<m|' p1 C1 st1 tm1 '~>' p2 C2 st2 tm2 '|m>'" := (MreachM p1 C1 st1 tm1 p2 C2 st2 tm2) 
+Notation "'<m|' C1 st1 tm1 '~>' C2 st2 tm2 '|m>'" := (MreachM C1 st1 tm1 C2 st2 tm2) 
                                                (at level 10, 
-                                                p1 at next level, C1 at next level, st1 at next level, tm1 at next level,
-                                                p2 at next level, C2 at next level, st2 at next level, tm2 at next level).
+                                                C1 at next level, st1 at next level, tm1 at next level,
+                                                C2 at next level, st2 at next level, tm2 at next level).
 
-Notation "'<e|' p1 C1 st1 tm1 '~>' p2 C2 st2 tm2 '|m>'" := (EreachM p1 C1 st1 tm1 p2 C2 st2 tm2) 
+Notation "'<e|' C1 st1 tm1 '~>' C2 st2 tm2 '|m>'" := (EreachM C1 st1 tm1 C2 st2 tm2) 
                                                (at level 10, 
-                                                p1 at next level, C1 at next level, st1 at next level, tm1 at next level,
-                                                p2 at next level, C2 at next level, st2 at next level, tm2 at next level).
+                                                C1 at next level, st1 at next level, tm1 at next level,
+                                                C2 at next level, st2 at next level, tm2 at next level).
 
 (* sanity check *)
-Lemma ere_trans : forall p1 C1 st1 e1
-                         p2 C2 st2 e2
-                         p3 C3 st3 e3
-                         (REACH1 : <e| p1 C1 st1 e1 ~> p2 C2 st2 e2 |e>)
-                         (REACH2 : <e| p2 C2 st2 e2 ~> p3 C3 st3 e3 |e>),
-                         <e| p1 C1 st1 e1 ~> p3 C3 st3 e3 |e>.
+Lemma ere_trans : forall C1 st1 e1
+                         C2 st2 e2
+                         C3 st3 e3
+                         (REACH1 : <e| C1 st1 e1 ~> C2 st2 e2 |e>)
+                         (REACH2 : <e| C2 st2 e2 ~> C3 st3 e3 |e>),
+                         <e| C1 st1 e1 ~> C3 st3 e3 |e>.
 Proof.
   intros. generalize dependent e3.
-  revert p3 C3 st3.
+  revert C3 st3.
   apply (_EreachE_ind_mut
-    (fun p1 C1 st1 e1 
-         p2 C2 st2 e2 
-         (REACH1 : <e| p1 C1 st1 e1 ~> p2 C2 st2 e2 |e>)=> 
-         forall p3 C3 st3 e3 
-                (REACH2 : <e| p2 C2 st2 e2 ~> p3 C3 st3 e3 |e>),
-                <e| p1 C1 st1 e1 ~> p3 C3 st3 e3 |e>)
-    (fun p1 C1 st1 e1 
-         p2 C2 st2 m2 
-         (REACH1 : <e| p1 C1 st1 e1 ~> p2 C2 st2 m2 |m>)=> 
-         forall p3 C3 st3 e3 
-                (REACH2 : <m| p2 C2 st2 m2 ~> p3 C3 st3 e3 |e>),
-                <e| p1 C1 st1 e1 ~> p3 C3 st3 e3 |e>)
-    (fun p1 C1 st1 m1
-         p2 C2 st2 e2
-         (REACH1 : <m| p1 C1 st1 m1 ~> p2 C2 st2 e2 |e>) =>
-         forall p3 C3 st3 e3 
-                (REACH2 : <e| p2 C2 st2 e2 ~> p3 C3 st3 e3 |e>),
-                <m| p1 C1 st1 m1 ~> p3 C3 st3 e3 |e>)
-    (fun p1 C1 st1 m1 
-         p2 C2 st2 m2 
-         (REACH1 : <m| p1 C1 st1 m1 ~> p2 C2 st2 m2 |m>)=> 
-         forall p3 C3 st3 e3 
-                (REACH2 : <m| p2 C2 st2 m2 ~> p3 C3 st3 e3 |e>),
-                <m| p1 C1 st1 m1 ~> p3 C3 st3 e3 |e>));
+    (fun C1 st1 e1 
+         C2 st2 e2 
+         (REACH1 : <e| C1 st1 e1 ~> C2 st2 e2 |e>)=> 
+         forall C3 st3 e3 
+                (REACH2 : <e| C2 st2 e2 ~> C3 st3 e3 |e>),
+                <e| C1 st1 e1 ~> C3 st3 e3 |e>)
+    (fun C1 st1 e1 
+         C2 st2 m2 
+         (REACH1 : <e| C1 st1 e1 ~> C2 st2 m2 |m>)=> 
+         forall C3 st3 e3 
+                (REACH2 : <m| C2 st2 m2 ~> C3 st3 e3 |e>),
+                <e| C1 st1 e1 ~> C3 st3 e3 |e>)
+    (fun C1 st1 m1
+         C2 st2 e2
+         (REACH1 : <m| C1 st1 m1 ~> C2 st2 e2 |e>) =>
+         forall C3 st3 e3 
+                (REACH2 : <e| C2 st2 e2 ~> C3 st3 e3 |e>),
+                <m| C1 st1 m1 ~> C3 st3 e3 |e>)
+    (fun C1 st1 m1 
+         C2 st2 m2 
+         (REACH1 : <m| C1 st1 m1 ~> C2 st2 m2 |m>)=> 
+         forall C3 st3 e3 
+                (REACH2 : <m| C2 st2 m2 ~> C3 st3 e3 |e>),
+                <m| C1 st1 m1 ~> C3 st3 e3 |e>));
    eauto using EreachE, EreachM, MreachE, MreachM;
    intros; try inversion pf; subst; inversion REACH2; subst;
    eauto using EreachE, EreachM, MreachE, MreachM.
 Qed.
 
-Lemma mrm_trans : forall p1 C1 st1 m1
-                         p2 C2 st2 m2
-                         p3 C3 st3 m3
-                         (REACH1 : <m| p1 C1 st1 m1 ~> p2 C2 st2 m2 |m>)
-                         (REACH2 : <m| p2 C2 st2 m2 ~> p3 C3 st3 m3 |m>),
-                         <m| p1 C1 st1 m1 ~> p3 C3 st3 m3 |m>.
+Lemma mrm_trans : forall C1 st1 m1
+                         C2 st2 m2
+                         C3 st3 m3
+                         (REACH1 : <m| C1 st1 m1 ~> C2 st2 m2 |m>)
+                         (REACH2 : <m| C2 st2 m2 ~> C3 st3 m3 |m>),
+                         <m| C1 st1 m1 ~> C3 st3 m3 |m>.
 Proof.
   intros. generalize dependent m3.
-  revert p3 C3 st3.
+  revert C3 st3.
   apply (_MreachM_ind_mut
-    (fun p1 C1 st1 e1 
-         p2 C2 st2 e2 
-         (REACH1 : <e| p1 C1 st1 e1 ~> p2 C2 st2 e2 |e>)=> 
-         forall p3 C3 st3 m3
-                (REACH2 : <e| p2 C2 st2 e2 ~> p3 C3 st3 m3 |m>),
-                <e| p1 C1 st1 e1 ~> p3 C3 st3 m3 |m>)
-    (fun p1 C1 st1 e1 
-         p2 C2 st2 m2 
-         (REACH1 : <e| p1 C1 st1 e1 ~> p2 C2 st2 m2 |m>)=> 
-         forall p3 C3 st3 m3 
-                (REACH2 : <m| p2 C2 st2 m2 ~> p3 C3 st3 m3 |m>),
-                <e| p1 C1 st1 e1 ~> p3 C3 st3 m3 |m>)
-    (fun p1 C1 st1 m1
-         p2 C2 st2 e2
-         (REACH1 : <m| p1 C1 st1 m1 ~> p2 C2 st2 e2 |e>) =>
-         forall p3 C3 st3 m3 
-                (REACH2 : <e| p2 C2 st2 e2 ~> p3 C3 st3 m3 |m>),
-                <m| p1 C1 st1 m1 ~> p3 C3 st3 m3 |m>)
-    (fun p1 C1 st1 m1 
-         p2 C2 st2 m2 
-         (REACH1 : <m| p1 C1 st1 m1 ~> p2 C2 st2 m2 |m>)=> 
-         forall p3 C3 st3 m3 
-                (REACH2 : <m| p2 C2 st2 m2 ~> p3 C3 st3 m3 |m>),
-                <m| p1 C1 st1 m1 ~> p3 C3 st3 m3 |m>));
+    (fun C1 st1 e1 
+         C2 st2 e2 
+         (REACH1 : <e| C1 st1 e1 ~> C2 st2 e2 |e>)=> 
+         forall C3 st3 m3 
+                (REACH2 : <e| C2 st2 e2 ~> C3 st3 m3 |m>),
+                <e| C1 st1 e1 ~> C3 st3 m3 |m>)
+    (fun C1 st1 e1 
+         C2 st2 m2 
+         (REACH1 : <e| C1 st1 e1 ~> C2 st2 m2 |m>)=> 
+         forall C3 st3 m3 
+                (REACH2 : <m| C2 st2 m2 ~> C3 st3 m3 |m>),
+                <e| C1 st1 e1 ~> C3 st3 m3 |m>)
+    (fun C1 st1 m1
+         C2 st2 e2
+         (REACH1 : <m| C1 st1 m1 ~> C2 st2 e2 |e>) =>
+         forall C3 st3 m3 
+                (REACH2 : <e| C2 st2 e2 ~> C3 st3 m3 |m>),
+                <m| C1 st1 m1 ~> C3 st3 m3 |m>)
+    (fun C1 st1 m1 
+         C2 st2 m2 
+         (REACH1 : <m| C1 st1 m1 ~> C2 st2 m2 |m>)=> 
+         forall C3 st3 m3 
+                (REACH2 : <m| C2 st2 m2 ~> C3 st3 m3 |m>),
+                <m| C1 st1 m1 ~> C3 st3 m3 |m>));
    eauto using EreachE, EreachM, MreachE, MreachM;
    intros; try inversion pf; subst; inversion REACH2; subst;
    eauto using EreachE, EreachM, MreachE, MreachM.
 Qed.
 
-Lemma ermre_trans : forall p1 C1 st1 e1
-                           p2 C2 st2 m2
-                           p3 C3 st3 e3
-                           (REACH1 : <e| p1 C1 st1 e1 ~> p2 C2 st2 m2 |m>)
-                           (REACH2 : <m| p2 C2 st2 m2 ~> p3 C3 st3 e3 |e>),
-                           <e| p1 C1 st1 e1 ~> p3 C3 st3 e3 |e>. 
+Lemma ermre_trans : forall C1 st1 e1
+                           C2 st2 m2
+                           C3 st3 e3
+                           (REACH1 : <e| C1 st1 e1 ~> C2 st2 m2 |m>)
+                           (REACH2 : <m| C2 st2 m2 ~> C3 st3 e3 |e>),
+                           <e| C1 st1 e1 ~> C3 st3 e3 |e>. 
 Proof.
   intros. generalize dependent e3.
-  revert p3 C3 st3.
+  revert C3 st3.
   apply (_EreachM_ind_mut
-    (fun p1 C1 st1 e1 
-         p2 C2 st2 e2 
-         (REACH1 : <e| p1 C1 st1 e1 ~> p2 C2 st2 e2 |e>)=> 
-         forall p3 C3 st3 e3 
-                (REACH2 : <e| p2 C2 st2 e2 ~> p3 C3 st3 e3 |e>),
-                <e| p1 C1 st1 e1 ~> p3 C3 st3 e3 |e>)
-    (fun p1 C1 st1 e1 
-         p2 C2 st2 m2 
-         (REACH1 : <e| p1 C1 st1 e1 ~> p2 C2 st2 m2 |m>)=> 
-         forall p3 C3 st3 e3 
-                (REACH2 : <m| p2 C2 st2 m2 ~> p3 C3 st3 e3 |e>),
-                <e| p1 C1 st1 e1 ~> p3 C3 st3 e3 |e>)
-    (fun p1 C1 st1 m1
-         p2 C2 st2 e2
-         (REACH1 : <m| p1 C1 st1 m1 ~> p2 C2 st2 e2 |e>) =>
-         forall p3 C3 st3 e3 
-                (REACH2 : <e| p2 C2 st2 e2 ~> p3 C3 st3 e3 |e>),
-                <m| p1 C1 st1 m1 ~> p3 C3 st3 e3 |e>)
-    (fun p1 C1 st1 m1 
-         p2 C2 st2 m2 
-         (REACH1 : <m| p1 C1 st1 m1 ~> p2 C2 st2 m2 |m>)=> 
-         forall p3 C3 st3 e3 
-                (REACH2 : <m| p2 C2 st2 m2 ~> p3 C3 st3 e3 |e>),
-                <m| p1 C1 st1 m1 ~> p3 C3 st3 e3 |e>));
+    (fun C1 st1 e1 
+         C2 st2 e2 
+         (REACH1 : <e| C1 st1 e1 ~> C2 st2 e2 |e>)=> 
+         forall C3 st3 e3 
+                (REACH2 : <e| C2 st2 e2 ~> C3 st3 e3 |e>),
+                <e| C1 st1 e1 ~> C3 st3 e3 |e>)
+    (fun C1 st1 e1 
+         C2 st2 m2 
+         (REACH1 : <e| C1 st1 e1 ~> C2 st2 m2 |m>)=> 
+         forall C3 st3 e3 
+                (REACH2 : <m| C2 st2 m2 ~> C3 st3 e3 |e>),
+                <e| C1 st1 e1 ~> C3 st3 e3 |e>)
+    (fun C1 st1 m1
+         C2 st2 e2
+         (REACH1 : <m| C1 st1 m1 ~> C2 st2 e2 |e>) =>
+         forall C3 st3 e3 
+                (REACH2 : <e| C2 st2 e2 ~> C3 st3 e3 |e>),
+                <m| C1 st1 m1 ~> C3 st3 e3 |e>)
+    (fun C1 st1 m1 
+         C2 st2 m2 
+         (REACH1 : <m| C1 st1 m1 ~> C2 st2 m2 |m>)=> 
+         forall C3 st3 e3 
+                (REACH2 : <m| C2 st2 m2 ~> C3 st3 e3 |e>),
+                <m| C1 st1 m1 ~> C3 st3 e3 |e>));
    eauto using EreachE, EreachM, MreachE, MreachM;
    intros; try inversion pf; subst; inversion REACH2; subst;
    eauto using EreachE, EreachM, MreachE, MreachM.
 Qed.
 
-Lemma mrerm_trans : forall p1 C1 st1 m1
-                           p2 C2 st2 e2
-                           p3 C3 st3 m3
-                           (REACH1 : <m| p1 C1 st1 m1 ~> p2 C2 st2 e2 |e>)
-                           (REACH2 : <e| p2 C2 st2 e2 ~> p3 C3 st3 m3 |m>),
-                           <m| p1 C1 st1 m1 ~> p3 C3 st3 m3 |m>. 
+Lemma mrerm_trans : forall C1 st1 m1
+                           C2 st2 e2
+                           C3 st3 m3
+                           (REACH1 : <m| C1 st1 m1 ~> C2 st2 e2 |e>)
+                           (REACH2 : <e| C2 st2 e2 ~> C3 st3 m3 |m>),
+                           <m| C1 st1 m1 ~> C3 st3 m3 |m>. 
 Proof.
   intros. generalize dependent m3.
-  revert p3 C3 st3.
+  revert C3 st3.
   apply (_MreachE_ind_mut
-    (fun p1 C1 st1 e1 
-         p2 C2 st2 e2 
-         (REACH1 : <e| p1 C1 st1 e1 ~> p2 C2 st2 e2 |e>)=> 
-         forall p3 C3 st3 m3
-                (REACH2 : <e| p2 C2 st2 e2 ~> p3 C3 st3 m3 |m>),
-                <e| p1 C1 st1 e1 ~> p3 C3 st3 m3 |m>)
-    (fun p1 C1 st1 e1 
-         p2 C2 st2 m2 
-         (REACH1 : <e| p1 C1 st1 e1 ~> p2 C2 st2 m2 |m>)=> 
-         forall p3 C3 st3 m3 
-                (REACH2 : <m| p2 C2 st2 m2 ~> p3 C3 st3 m3 |m>),
-                <e| p1 C1 st1 e1 ~> p3 C3 st3 m3 |m>)
-    (fun p1 C1 st1 m1
-         p2 C2 st2 e2
-         (REACH1 : <m| p1 C1 st1 m1 ~> p2 C2 st2 e2 |e>) =>
-         forall p3 C3 st3 m3 
-                (REACH2 : <e| p2 C2 st2 e2 ~> p3 C3 st3 m3 |m>),
-                <m| p1 C1 st1 m1 ~> p3 C3 st3 m3 |m>)
-    (fun p1 C1 st1 m1 
-         p2 C2 st2 m2 
-         (REACH1 : <m| p1 C1 st1 m1 ~> p2 C2 st2 m2 |m>)=> 
-         forall p3 C3 st3 m3 
-                (REACH2 : <m| p2 C2 st2 m2 ~> p3 C3 st3 m3 |m>),
-                <m| p1 C1 st1 m1 ~> p3 C3 st3 m3 |m>));
+    (fun C1 st1 e1 
+         C2 st2 e2 
+         (REACH1 : <e| C1 st1 e1 ~> C2 st2 e2 |e>)=> 
+         forall C3 st3 m3 
+                (REACH2 : <e| C2 st2 e2 ~> C3 st3 m3 |m>),
+                <e| C1 st1 e1 ~> C3 st3 m3 |m>)
+    (fun C1 st1 e1 
+         C2 st2 m2 
+         (REACH1 : <e| C1 st1 e1 ~> C2 st2 m2 |m>)=> 
+         forall C3 st3 m3 
+                (REACH2 : <m| C2 st2 m2 ~> C3 st3 m3 |m>),
+                <e| C1 st1 e1 ~> C3 st3 m3 |m>)
+    (fun C1 st1 m1
+         C2 st2 e2
+         (REACH1 : <m| C1 st1 m1 ~> C2 st2 e2 |e>) =>
+         forall C3 st3 m3 
+                (REACH2 : <e| C2 st2 e2 ~> C3 st3 m3 |m>),
+                <m| C1 st1 m1 ~> C3 st3 m3 |m>)
+    (fun C1 st1 m1 
+         C2 st2 m2 
+         (REACH1 : <m| C1 st1 m1 ~> C2 st2 m2 |m>)=> 
+         forall C3 st3 m3 
+                (REACH2 : <m| C2 st2 m2 ~> C3 st3 m3 |m>),
+                <m| C1 st1 m1 ~> C3 st3 m3 |m>));
    eauto using EreachE, EreachM, MreachE, MreachM;
    intros; try inversion pf; subst; inversion REACH2; subst;
    eauto using EreachE, EreachM, MreachE, MreachM.
@@ -827,110 +689,125 @@ Lemma c_plugin_assoc : forall C1 C2 C3, C1[| C2[| C3 |] |] = ((C1[|C2|])[|C3|]).
 Proof.
   induction C1; eauto; 
   intros; simpl; try rewrite IHC1; eauto.
+  rewrite IHC1_2. eauto.
 Qed.
 
-Lemma c_plugin_adds_level : forall C1 C2, level(C1[|C2|]) = level C1 + level C2.
+Lemma eq_p_eq : forall p1 p2, eq_p p1 p2 = true <-> p1 = p2.
 Proof.
-  induction C1; eauto;
-  intros; simpl; try rewrite IHC1; eauto.
+  induction p1; induction p2;
+  intros; simpl;
+  try rewrite IHp1; try rewrite IHp2;
+  eauto.
+  - split; eauto.
+  - split; intros contra; inversion contra.
+  - split; intros contra; inversion contra.
+  - unfold eq_t. remember (a =? a0) as eqa.
+    destruct eqa; simpl; symmetry in Heqeqa;
+    try rewrite Nat.eqb_eq in Heqeqa;
+    try rewrite Nat.eqb_neq in Heqeqa.
+    + split; intros. rewrite Heqeqa in *.
+      apply IHp1 in H. rewrite H. eauto.
+      eapply IHp1. inversion H; eauto.
+    + split; intros contra; inversion contra.
+      apply Heqeqa in H0; inversion H0.
+Qed.
+
+Lemma c_plugin_adds_level : forall C1 C2, eq_p (dy_level(C1[|C2|])) (dy_level C1 ++ dy_level C2) = true.
+Proof.
+  induction C1; induction C2;
+  intros; simpl; 
+  try rewrite IHC1; try rewrite IHC2; try unfold eq_t;
+  eauto; try (assert (RR : tx =? tx = true);
+  try apply Nat.eqb_eq; eauto; try rewrite RR; try clear RR; eauto).
+  - assert (RR : dy_level (dy_c_letm M C2_1 C2_2) = dy_level C2_2); eauto;
+    rewrite <- RR; clear RR; eapply IHC1.
+  - assert (RR : dy_level (dy_c_letm M C2_1 C2_2) = dy_level C2_2); eauto;
+    rewrite <- RR; clear RR; eapply IHC1.
+  - assert (RR : dy_level (dy_c_letm M0 C2_1 C2_2) = dy_level C2_2); eauto;
+    rewrite <- RR; clear RR; eapply IHC1_2.
 Qed.
 
 (* equivalence between reachability relations *)
 Lemma Eeval_then_reach :
-    forall pi Ci sti ei v stv
-           (EVAL : EevalR pi Ci sti ei v stv)
-           ev pf pv Cv e_mem m_mem t
-           (VAL : v = Val ev pf pv Cv)
-           (STATE : stv = ST e_mem m_mem t),
-          <e| pi Ci sti ei ~> pv Cv stv ev |e>.
+    forall Ci sti ei v stv
+           (EVAL : EevalR Ci sti ei v stv)
+           ev pf Cv mem t
+           (VAL : v = Val ev pf Cv)
+           (STATE : stv = ST mem t),
+          <e| Ci sti ei ~> Cv stv ev |e>.
 Proof.
   apply (EevalR_ind_mut
-    (fun pi Ci sti ei v stv
-        (EVAL : EevalR pi Ci sti ei v stv) =>
-        forall ev pf pv Cv e_mem m_mem t
-              (VAL : v = Val ev pf pv Cv)
-              (STATE : stv = ST e_mem m_mem t),
-        <e| pi Ci sti ei ~> pv Cv stv ev |e>)
-    (fun pi Ci sti mi v stv
-        (EVAL : MevalR pi Ci sti mi v stv) =>
-        forall pv Cv e_mem m_mem t
-              (VAL : v = Mod pv Cv)
-              (STATE : stv = ST e_mem m_mem t),
-        <m| pi Ci sti mi ~> pv Cv stv m_empty |m>));
+    (fun Ci sti ei v stv
+        (EVAL : EevalR Ci sti ei v stv) =>
+        forall ev pf Cv mem t
+              (VAL : v = Val ev pf Cv)
+              (STATE : stv = ST mem t),
+        <e| Ci sti ei ~> Cv stv ev |e>)
+    (fun Ci sti mi Cv stv
+        (EVAL : MevalR Ci sti mi Cv stv) =>
+        <m| Ci sti mi ~> Cv stv m_empty |m>));
   intros; try inversion STATE0; try inversion STATE;
           try inversion VAL; try destruct st_lam;
           try destruct st_m; try destruct v_e;
           try destruct v_m1; try destruct arg; subst; 
           eauto using EreachE, EreachM, MreachE, MreachM.
-  - inversion STATE; subst. destruct st; subst.
-    eapply mrm_lete_m. eapply EVALe.
-    eapply H. eauto. eauto. eapply H0. eauto. eauto.
 Qed.
 
 Lemma Meval_then_reach :
-    forall pi Ci sti mi v stv
-           (EVAL : MevalR pi Ci sti mi v stv)
-           pv Cv e_mem m_mem t
-           (VAL : v = Mod pv Cv)
-           (STATE : stv = ST e_mem m_mem t),
-           <m| pi Ci sti mi ~> pv Cv stv m_empty |m>.
+    forall Ci sti mi Cv stv
+           (EVAL : MevalR Ci sti mi Cv stv),
+           <m| Ci sti mi ~> Cv stv m_empty |m>.
 Proof.
   apply (MevalR_ind_mut
-    (fun pi Ci sti ei v stv
-        (EVAL : EevalR pi Ci sti ei v stv) =>
-        forall ev pf pv Cv e_mem m_mem t
-              (VAL : v = Val ev pf pv Cv)
-              (STATE : stv = ST e_mem m_mem t),
-        <e| pi Ci sti ei ~> pv Cv stv ev |e>)
-    (fun pi Ci sti mi v stv
-        (EVAL : MevalR pi Ci sti mi v stv) =>
-        forall pv Cv e_mem m_mem t
-              (VAL : v = Mod pv Cv)
-              (STATE : stv = ST e_mem m_mem t),
-        <m| pi Ci sti mi ~> pv Cv stv m_empty |m>));
+    (fun Ci sti ei v stv
+        (EVAL : EevalR Ci sti ei v stv) =>
+        forall ev pf Cv mem t
+              (VAL : v = Val ev pf Cv)
+              (STATE : stv = ST mem t),
+        <e| Ci sti ei ~> Cv stv ev |e>)
+    (fun Ci sti mi Cv stv
+        (EVAL : MevalR Ci sti mi Cv stv) =>
+        <m| Ci sti mi ~> Cv stv m_empty |m>));
   intros; try inversion STATE0; try inversion STATE;
           try inversion VAL; try destruct st_lam;
           try destruct st_m; try destruct v_e;
           try destruct v_m1; try destruct arg; subst; 
           eauto using EreachE, EreachM, MreachE, MreachM.
-  - inversion STATE; subst. destruct st; subst.
-    eapply mrm_lete_m. eapply EVALe.
-    eapply H. eauto. eauto. eapply H0. eauto. eauto.
 Qed.
 
 Lemma EreachE_equiv_left :
-    forall p1 C1 st1 e1 p2 C2 st2 e2,
-          <e| p1 C1 st1 e1 ~> p2 C2 st2 e2 |e> ->
-          _EreachE p1 C1 st1 e1 p2 C2 st2 e2.
+    forall C1 st1 e1 C2 st2 e2,
+          <e| C1 st1 e1 ~> C2 st2 e2 |e> ->
+          _EreachE C1 st1 e1 C2 st2 e2.
 Proof.
   apply (_EreachE_ind_mut 
-    (fun p1 C1 st1 e1 p2 C2 st2 e2
-        (REACH : <e| p1 C1 st1 e1 ~> p2 C2 st2 e2 |e>) =>
-        _EreachE p1 C1 st1 e1 p2 C2 st2 e2)
-    (fun p1 C1 st1 e1 p2 C2 st2 m2
-        (REACH : <e| p1 C1 st1 e1 ~> p2 C2 st2 m2 |m>) =>
-        _EreachM p1 C1 st1 e1 p2 C2 st2 m2)
-    (fun p1 C1 st1 m1 p2 C2 st2 e2
-        (REACH : <m| p1 C1 st1 m1 ~> p2 C2 st2 e2 |e>) =>
-        _MreachE p1 C1 st1 m1 p2 C2 st2 e2)
-    (fun p1 C1 st1 m1 p2 C2 st2 m2
-        (REACH : <m| p1 C1 st1 m1 ~> p2 C2 st2 m2 |m>) =>
-        _MreachM p1 C1 st1 m1 p2 C2 st2 m2));
+    (fun C1 st1 e1 C2 st2 e2
+        (REACH : <e| C1 st1 e1 ~> C2 st2 e2 |e>) =>
+        _EreachE C1 st1 e1 C2 st2 e2)
+    (fun C1 st1 e1 C2 st2 m2
+        (REACH : <e| C1 st1 e1 ~> C2 st2 m2 |m>) =>
+        _EreachM C1 st1 e1 C2 st2 m2)
+    (fun C1 st1 m1 C2 st2 e2
+        (REACH : <m| C1 st1 m1 ~> C2 st2 e2 |e>) =>
+        _MreachE C1 st1 m1 C2 st2 e2)
+    (fun C1 st1 m1 C2 st2 m2
+        (REACH : <m| C1 st1 m1 ~> C2 st2 m2 |m>) =>
+        _MreachM C1 st1 m1 C2 st2 m2));
   intros; eauto using EreachE, EreachM, MreachE, MreachM, _EreachE, _MreachE, _EreachM, _MreachM.
 Qed.
 
 Lemma EreachE_equiv_right :
-    forall p1 C1 st1 e1 p2 C2 st2 e2,
-          _EreachE p1 C1 st1 e1 p2 C2 st2 e2 ->
-          <e| p1 C1 st1 e1 ~> p2 C2 st2 e2 |e>.
+    forall C1 st1 e1 C2 st2 e2,
+          _EreachE C1 st1 e1 C2 st2 e2 ->
+          <e| C1 st1 e1 ~> C2 st2 e2 |e>.
 Proof.
   apply (__EreachE_ind_mut 
-    (fun p1 C1 st1 e1 p2 C2 st2 e2
-        (REACH : _EreachE p1 C1 st1 e1 p2 C2 st2 e2) =>
-        <e| p1 C1 st1 e1 ~> p2 C2 st2 e2 |e>)
-    (fun p1 C1 st1 m1 p2 C2 st2 e2
-        (REACH : _MreachE p1 C1 st1 m1 p2 C2 st2 e2) =>
-        <m| p1 C1 st1 m1 ~> p2 C2 st2 e2 |e>));
+    (fun C1 st1 e1 C2 st2 e2
+        (REACH : _EreachE C1 st1 e1 C2 st2 e2) =>
+        <e| C1 st1 e1 ~> C2 st2 e2 |e>)
+    (fun C1 st1 m1 C2 st2 e2
+        (REACH : _MreachE C1 st1 m1 C2 st2 e2) =>
+        <m| C1 st1 m1 ~> C2 st2 e2 |e>));
   intros; try destruct v; try destruct st; try destruct st1; try destruct st_lam;
   try destruct arg; try destruct st_m; try destruct st';
   eauto using EreachE, EreachM, MreachE, MreachM, _EreachE, _MreachE, _EreachM, _MreachM.
@@ -943,236 +820,374 @@ Proof.
 Qed.
 
 Theorem EreachE_equiv : 
-  forall p1 C1 st1 e1 p2 C2 st2 e2,
-          _EreachE p1 C1 st1 e1 p2 C2 st2 e2 <->
-          <e| p1 C1 st1 e1 ~> p2 C2 st2 e2 |e>.
+  forall C1 st1 e1 C2 st2 e2,
+         _EreachE C1 st1 e1 C2 st2 e2 <->
+          <e| C1 st1 e1 ~> C2 st2 e2 |e>.
 Proof. 
   intros; split; try apply EreachE_equiv_left; try apply EreachE_equiv_right. 
 Qed.
 
-(* Induction principle: preserves a predicate on p, C, st *)
-Lemma EreachE_ind_mut : 
-  forall (P : forall (p : path) (C : ctx) (st : state), Prop),
-    (forall p C st, (P p C st) -> 
-        (match st with
-        | ST e_mem m_mem _ =>
-            forall addr,
-            match e_mem addr with
-              | None => True
-              | Some (Val _ _ p' C') => P p' C' st
-            end /\
-            match m_mem addr with
-              | None => True
-              | Some (Mod p' C') => P p' C' st
-            end
-        end)) ->
-    (forall p C st p' C' st'
-            (INIT : P p C st)
-            (REACH : P p' C' st'),
-            P p C st') ->
-    (forall p C st 
-            x p_lam C_lam st_lam 
-            v pf p_arg C_arg e_mem m_mem t
-            (INIT : P p C st)
-            (FN: P p_lam C_lam st_lam)
-            (ARG : P p_arg C_arg (ST e_mem m_mem t)),
-            P (t :: p_lam) (C_lam[|c_lam x c_hole|])
-              (ST ((t :: p_lam) !-> (Val v pf p_arg C_arg); e_mem) m_mem (update_t t))) ->
-    (forall p C st x
-            v (pf : value v) p_x C_x e_mem m_mem t
-            (INIT : P p C st)
-            (EVx : P p_x C_x (ST e_mem m_mem t)),
-            P (t :: p) (C[|c_lete x c_hole|])
-              (ST ((t :: p) !-> (Val v pf p_x C_x); e_mem) m_mem (update_t t))) ->
-    (forall p C st M
-            p_M C_M e_mem m_mem t
-            (INIT : P p C st)
-            (EVM : P p_M C_M (ST e_mem m_mem t)),
-            P (t :: p) (C[|c_letm M c_hole|])
-              (ST e_mem ((t :: p) !-> (Mod p_M C_M); m_mem) (update_t t))) ->
-    (forall p C st e p' C' st' e'
-            (INIT : P p C st)
-            (REACH : <e| p C st e ~> p' C' st' e' |e>),
-            P p' C' st').
-Proof. 
-(* intros just before our goal, then fix 10, on REACH, 
-   with mutual induction on EreachM, MreachE, MreachM *)
-  intros P condP transP LAM LETe LETm.
-  fix IHere 10 with 
-    (IHerm p C st e p' C' st' m'
-          (INIT : P p C st)
-          (REACH : <e| p C st e ~> p' C' st' m' |m>)
-          { struct REACH }
-          : P p' C' st')
-    (IHmre p C st m p' C' st' e'
-          (INIT : P p C st)
-          (REACH : <m| p C st m ~> p' C' st' e' |e>)
-          { struct REACH }
-          : P p' C' st')
-    (IHmrm p C st m p' C' st' m'
-          (INIT : P p C st)
-          (REACH : <m| p C st m ~> p' C' st' m' |m>)
-          { struct REACH }
-          : P p' C' st').
-  - intros. destruct REACH.
-    + exact INIT.
-    + specialize (condP p C st INIT).
-      rewrite <- STATE in *. destruct (condP p_x) as [valcase modcase].
-      rewrite <- ACCESS in *. exact valcase.
-    + apply (IHere p C st e1 p' C' st' e'). exact INIT. exact REACH.
-    + apply (IHere p C st1 e2 p' C' st' e').
-      assert (P p1 C1 st1) as trans.
-      apply (IHere p C st e1 p1 C1 st1 v).
-      exact INIT. exact REACH1. eapply transP.
-      exact INIT. exact trans. exact REACH2.
-    + apply (IHere (t :: p_lam) (C_lam [|c_lam x c_hole|])
-            (ST (t :: p_lam !-> (Val arg pf p_arg C_arg); e_mem) m_mem (update_t t)) e
-            p' C' st' e').
-      assert (P p_lam C_lam st_lam) as trans.
-      apply (IHere p C st e1 p_lam C_lam st_lam (e_lam x e)).
-      exact INIT. exact REACH1.
-      apply LAM with (p := p) (C := C) (st := st) (st_lam := st_lam).
-      exact INIT. exact trans. apply (IHere p C st_lam e2 p_arg C_arg (ST e_mem m_mem t) arg).
-      eapply transP. eapply INIT. eapply trans. apply REACH2. exact REACH3.
-    + apply (IHmre p C st m p' C' st' e'). exact INIT. exact REACHm.
-    + apply (IHere p_m C_m st_m e p' C' st' e').
-      apply (IHmrm p C st m p_m C_m st_m m_empty).
-      exact INIT. exact MODr. exact REACH.
-  - intros. destruct REACH.
-    + apply (IHerm p C st e1 p' C' st' m'). exact INIT. exact REACH.
-    + apply (IHerm p C st1 e2 p' C' st' m').
-      assert (P p1 C1 st1) as trans.
-      apply (IHere p C st e1 p1 C1 st1 v).
-      exact INIT. exact FNr. eapply transP.
-      exact INIT. exact trans. exact REACH.
-    + apply (IHerm (t :: p_lam) (C_lam [|c_lam x c_hole|])
-            (ST (t :: p_lam !-> Val arg pf p_arg C_arg; e_mem) m_mem (update_t t)) e
-            p' C' st' m').
-      assert (P p_lam C_lam st_lam) as trans.
-      apply (IHere p C st e1 p_lam C_lam st_lam (e_lam x e)).
-      exact INIT. exact FNr.
-      apply LAM with (p := p) (C := C) (st := st) (st_lam := st_lam).
-      exact INIT. exact trans. apply (IHere p C st_lam e2 p_arg C_arg (ST e_mem m_mem t) arg).
-      eapply transP. eapply INIT. eapply trans. apply ARGr. exact REACH.
-    + apply (IHmrm p C st m p' C' st' m'). exact INIT. exact REACHm.
-    + apply (IHerm p_m C_m st_m e p' C' st' m').
-      apply (IHmrm p C st m p_m C_m st_m m_empty).
-      exact INIT. exact MODr. exact REACH.
-  - intros. destruct REACH.
-    + apply (IHere p C st e p' C' st' e'). exact INIT. exact REACHe.
-    + apply (IHmre (t :: p) (C [|c_lete x c_hole|])
-        (ST (t :: p !-> Val v pf p1 C1; e_mem) m_mem (update_t t)) m
-        p' C' st' e').
-      eapply LETe. exact INIT. apply (IHere p C st e p1 C1 (ST e_mem m_mem t) v).
-      exact INIT. exact EVALxr. exact REACH.
-    + apply (IHmre p C st m1 p' C' st' e'). exact INIT. exact REACH.
-    + apply (IHmre (t :: p) (C [|c_letm M c_hole|])
-        (ST e_mem (t :: p !-> Mod p_m C_m; m_mem) (update_t t)) m2 p'
-        C' st' e' ).
-      eapply LETm. exact INIT. apply (IHmrm p C st m1 p_m C_m (ST e_mem m_mem t) m_empty).
-      exact INIT. exact EVALMr. exact REACH.
-  - intros. destruct REACH.
-    + exact INIT.
-    + specialize (condP p C st INIT).
-      rewrite <- STATE in *. destruct (condP p_M) as [valcase modcase].
-      rewrite <- ACCESS in *. exact modcase.
-    + apply (IHerm p C st e p' C' st' m'). exact INIT. exact REACHe.
-    + apply (IHmrm (t :: p) (C [|c_lete x c_hole|])
-        (ST (t :: p !-> Val v pf p1 C1; e_mem) m_mem (update_t t)) m
-        p' C' st' m').
-      eapply LETe. exact INIT. apply (IHere p C st e p1 C1 (ST e_mem m_mem t) v).
-      exact INIT. exact EVALxr. exact REACH.
-    + apply (IHmrm p C st m1 p' C' st' m'). exact INIT. exact REACH.
-    + apply (IHmrm (t :: p) (C [|c_letm M c_hole|])
-        (ST e_mem (t :: p !-> Mod p_m C_m; m_mem) (update_t t)) m2 p'
-        C' st' m' ).
-      eapply LETm. exact INIT. apply (IHmrm p C st m1 p_m C_m (ST e_mem m_mem t) m_empty).
-      exact INIT. exact REACH1. exact REACH2.
+Inductive st_ctx :=
+  | st_c_hole
+  | st_c_lam (x : expr_id) (C : st_ctx)
+  | st_c_lete (x : expr_id) (C : st_ctx)
+  | st_c_letm (M : mod_id) (CM : st_ctx) (C : st_ctx)
+.
+
+Fixpoint st_level (C : st_ctx) : nat :=
+  match C with
+  | st_c_hole => 0
+  | st_c_lam _ C'
+  | st_c_lete _ C' => S (st_level C')
+  | st_c_letm _ _ C' => st_level C'
+  end.
+
+Fixpoint st_ctx_M (C : st_ctx) (M : mod_id) :=
+  match C with
+  | st_c_hole => None
+  | st_c_lam _ C'
+  | st_c_lete _ C' => st_ctx_M C' M
+  | st_c_letm M' CM' C' =>
+    match st_ctx_M C' M with
+    | Some CM => Some CM
+    | None => if eq_mid M M' then Some CM' else None
+    end
+  end.
+
+Fixpoint st_c_plugin (Cout : st_ctx) (Cin : st_ctx) :=
+  match Cout with
+  | st_c_hole => Cin
+  | st_c_lam x C' => st_c_lam x (st_c_plugin C' Cin)
+  | st_c_lete x C' => st_c_lete x (st_c_plugin C' Cin)
+  | st_c_letm M' CM' C' => st_c_letm M' CM' (st_c_plugin C' Cin)
+  end.
+
+(* given a static context and an expression, 
+   return the maximum level of the context
+   that can be reached from here *)
+Fixpoint level_expr (C : st_ctx) e :=
+  match e with
+  | e_var x => st_level C
+  | e_lam x e' => level_expr (st_c_plugin C (st_c_lam x st_c_hole)) e'
+  | e_app e1 e2 => Nat.max (level_expr C e1) (level_expr C e2)
+  | e_link m e =>
+    match level_mod C m with
+    | (Some C_m, l) => Nat.max (level_expr C_m e) l
+    | (None, l) => l
+    end
+  end
+
+with level_mod (C : st_ctx) m :=
+  match m with
+  | m_empty => (Some C, st_level C)
+  | m_var M =>
+    match st_ctx_M C M with
+    | None => (None, st_level C)
+    | Some C_m => (Some C_m, Nat.max (st_level C) (st_level C_m))
+    end
+  | m_lete x e m' => 
+    match level_expr C e with
+    | l_e => 
+      match level_mod (st_c_plugin C (st_c_lete x st_c_hole)) m' with
+      | (context, l_m) => (context, Nat.max l_e l_m)
+      end
+    end
+  | m_letm M m1 m2 =>
+    match level_mod C m1 with
+    | (Some C_m, l1) =>
+      match level_mod (st_c_plugin C (st_c_letm M C_m st_c_hole)) m2 with
+      | (context, l2) => (context, Nat.max l1 l2)
+      end
+    | (None, l1) => (None, l1)
+    end
+  end.
+
+Lemma st_c_plugin_add_level :
+  forall C1 C2, st_level (st_c_plugin C1 C2) = st_level C1 + st_level C2.
+Proof.
+  induction C1; induction C2; intros; simpl; eauto.
+  - assert (RR : st_level (st_c_letm M C2_1 C2_2) = st_level C2_2); eauto.
+    specialize (IHC1 (st_c_letm M C2_1 C2_2)).
+    rewrite IHC1. rewrite RR. eauto.
+  - assert (RR : st_level (st_c_letm M C2_1 C2_2) = st_level C2_2); eauto.
+    specialize (IHC1 (st_c_letm M C2_1 C2_2)).
+    rewrite IHC1. rewrite RR. eauto.
+  - assert (RR : st_level (st_c_letm M0 C2_1 C2_2) = st_level C2_2); eauto.
+    specialize (IHC1_2 (st_c_letm M0 C2_1 C2_2)).
+    rewrite IHC1_2. rewrite RR. eauto.
 Qed.
 
-Definition st_len m n p C st :=
+(* sanity check *)
+Lemma level_increase : forall e C, st_level C <= level_expr C e.
+Proof.
+  apply (expr_ind_mut
+    (fun e =>
+      forall C, st_level C <= level_expr C e)
+    (fun m =>
+      forall C, 
+      match level_mod C m with
+        | (_, l) => st_level C <= l
+      end)); 
+  intros; simpl in *; try nia.
+  induction C; intros; simpl in *; try nia.
+  - assert (RR : st_level (st_c_lam x0 (st_c_plugin C (st_c_lam x st_c_hole))) =
+            S (S(st_level C))); simpl; try rewrite st_c_plugin_add_level; simpl; try nia;
+      assert (middle : S (S (st_level C)) <= level_expr (st_c_lam x0 (st_c_plugin C (st_c_lam x st_c_hole))) e);
+      try rewrite <- RR; try apply H; try nia.
+  - assert (RR : st_level (st_c_lete x0 (st_c_plugin C (st_c_lam x st_c_hole))) =
+            S (S(st_level C))); simpl; try rewrite st_c_plugin_add_level; simpl; try nia;
+    assert (middle : S (S (st_level C)) <= level_expr (st_c_lete x0 (st_c_plugin C (st_c_lam x st_c_hole))) e);
+    try rewrite <- RR; try apply H; try nia.
+  - assert (RR : st_level (st_c_letm M C1 (st_c_plugin C2 (st_c_lam x st_c_hole))) =
+            (st_level C2) + 1); simpl; repeat try rewrite st_c_plugin_add_level; simpl; eauto; try nia.
+    assert (middle : (st_level C2) + 1 <= level_expr (st_c_letm M C1 (st_c_plugin C2 (st_c_lam x st_c_hole))) e);
+    try rewrite <- RR; try apply H; try nia.
+  - specialize (H C). specialize (H0 C). nia.
+  - remember (level_mod C m) as ol. destruct ol.
+    destruct o; specialize (H C); rewrite <- Heqol in H; nia.
+  - remember (st_ctx_M C M) as o. destruct o; nia.
+  - remember (level_mod (st_c_plugin C (st_c_lete x st_c_hole)) m) as ol. destruct ol.
+    specialize (H0 (st_c_plugin C (st_c_lete x st_c_hole))). rewrite <- Heqol in H0.
+    rewrite st_c_plugin_add_level in H0. simpl in H0. nia.
+  - remember (level_mod C m1) as ol1. destruct ol1.
+    destruct o;
+    try remember (level_mod (st_c_plugin C (st_c_letm M s st_c_hole)) m2) as ol2; try destruct ol2;
+    try specialize (H C); eauto; try specialize (H0 (st_c_plugin C (st_c_letm M s st_c_hole)));
+    rewrite <- Heqol1 in H; try rewrite <- Heqol2 in H0;
+    try rewrite st_c_plugin_add_level in H0; try simpl in H0; try nia.
+Qed.
+
+Fixpoint dy_to_st C :=
+  match C with
+  | dy_c_hole => st_c_hole
+  | dy_c_lam x _ C' => st_c_lam x (dy_to_st C')
+  | dy_c_lete x _ C' => st_c_lete x (dy_to_st C')
+  | dy_c_letm M CM C' => st_c_letm M (dy_to_st CM) (dy_to_st C')
+  end.
+
+Lemma dy_to_st_plugin :
+  forall Cout Cin,
+    dy_to_st (Cout[|Cin|]) = st_c_plugin (dy_to_st Cout) (dy_to_st Cin).
+Proof.
+  induction Cout; intros; simpl; try rewrite IHCout; eauto.
+  rewrite IHCout2. eauto.
+Qed. 
+
+Lemma mod_is_static_none : forall (dC : dy_ctx) (M : mod_id),
+  (ctx_M dC M = None <-> st_ctx_M (dy_to_st dC) M = None).
+Proof. 
+  intros. repeat split. 
+  - induction dC; simpl; eauto.
+    destruct (ctx_M dC2 M). intros H; inversion H.
+    specialize (IHdC2 eq_refl). rewrite IHdC2.
+    destruct (eq_mid M M0). intros H; inversion H. eauto.
+  - induction dC; simpl; eauto.
+    destruct (st_ctx_M (dy_to_st dC2) M). intros H; inversion H.
+    specialize (IHdC2 eq_refl). rewrite IHdC2.
+    destruct (eq_mid M M0). intros H; inversion H. eauto.
+Qed.
+
+Lemma mod_is_static_some : forall (dC : dy_ctx) (M : mod_id),
+  (forall v, ctx_M dC M = Some v -> st_ctx_M (dy_to_st dC) M = Some (dy_to_st v)) /\
+  (forall v, st_ctx_M (dy_to_st dC) M = Some v -> exists dv, dy_to_st dv = v /\ ctx_M dC M = Some dv).
+Proof.
+  intros; split. 
+  - induction dC; simpl; intros; eauto.
+    + inversion H.
+    + remember (ctx_M dC2 M) as v2. destruct v2.
+      specialize (IHdC2 v H). rewrite IHdC2. eauto.
+      symmetry in Heqv2. rewrite mod_is_static_none in Heqv2.
+      rewrite Heqv2. destruct (eq_mid M M0); inversion H; eauto.
+  - induction dC; simpl; intros; eauto.
+    + inversion H.
+    + remember (st_ctx_M (dy_to_st dC2) M) as v2. destruct v2.
+      specialize (IHdC2 v H). inversion IHdC2. exists x.
+      destruct H0. split. assumption. rewrite H1. eauto.
+      remember (ctx_M dC2 M) as v2. destruct v2;
+      symmetry in Heqv2; rewrite <- mod_is_static_none in Heqv2.
+      rewrite Heqv2 in Heqv0. inversion Heqv0.
+      destruct (eq_mid M M0). inversion H.
+      exists dC1. eauto. inversion H.
+Qed.
+
+(* Induction principle: preserves a predicate on C, st, e *)
+Lemma EreachE_ind_mut : 
+  forall (Pe : forall (C : dy_ctx) (st : state) (e : expr_tm), Prop)
+         (Pm : forall (C : dy_ctx) (st : state) (m : mod_tm), Prop),
+    (forall C st e, (Pe C st e) -> 
+      (match st with
+      | ST mem _ =>
+          forall addr,
+          match mem addr with
+            | None => True
+            | Some (Val v _ C') => Pe C' st v
+          end
+      end)) ->
+    (forall C st e1 e2,
+            Pe C st (e_app e1 e2) -> Pe C st e1) ->
+    (forall C st e1 e2 C_lam st_lam lam,
+            Pe C st (e_app e1 e2) -> 
+            Pe C_lam st_lam lam -> Pe C st_lam e2) ->
+    (forall C st e1 e2 C_lam st_lam x e
+            C_arg mem t arg pf,
+            Pe C st (e_app e1 e2) ->
+            Pe C_lam st_lam (e_lam x e) ->
+            Pe C_arg (ST mem t) arg ->
+            Pe (C_lam[|dy_c_lam x t dy_c_hole|])
+              (ST ((dy_level C_lam ++ [t]) !-> (Val arg pf C_arg) ; mem) (update_t t)) e) ->
+    (forall C st m e, Pe C st (e_link m e) -> Pm C st m) ->
+    (forall C st m e C_m st_m,
+            Pe C st (e_link m e) ->
+            Pm C_m st_m m_empty -> Pe C_m st_m e) ->
+    (forall C st M C_M (ACCESS : Some C_M = ctx_M C M),
+            Pm C st (m_var M) -> Pm C_M st m_empty) ->
+    (forall C st x e m,
+            Pm C st (m_lete x e m) -> Pe C st e) ->
+    (forall C st x e m C_x mem t v pf,
+            Pm C st (m_lete x e m) ->
+            Pe C_x (ST mem t) v ->
+            Pm (C[|dy_c_lete x t dy_c_hole|])
+              (ST ((dy_level C ++ [t]) !-> (Val v pf C_x) ; mem) (update_t t)) m) ->
+    (forall C st M m1 m2,
+            Pm C st (m_letm M m1 m2) -> Pm C st m1) ->
+    (forall C st M m1 m2 C_M st_M,
+            Pm C st (m_letm M m1 m2) ->
+            Pm C_M st_M m_empty ->
+            Pm (C[|dy_c_letm M C_M dy_c_hole|]) st_M m2) ->
+    (forall C st e C' st' e'
+            (INIT : Pe C st e)
+            (REACH : <e| C st e ~> C' st' e' |e>),
+            Pe C' st' e').
+Proof. 
+(* intros just before our goal, then fix 8, on REACH, 
+   with mutual induction on EreachM, MreachE, MreachM *)
+  intros Pe Pm MEM APPl APPr APPb LINKm LINKe MVAR LETex LETem LETm1 LETm2.
+  fix IHere 8 with 
+    (IHerm C st e C' st' m'
+          (INIT : Pe C st e)
+          (REACH : <e| C st e ~> C' st' m' |m>)
+          { struct REACH }
+          : Pm C' st' m')
+    (IHmre C st m C' st' e'
+          (INIT : Pm C st m)
+          (REACH : <m| C st m ~> C' st' e' |e>)
+          { struct REACH }
+          : Pe C' st' e')
+    (IHmrm C st m C' st' m'
+          (INIT : Pm C st m)
+          (REACH : <m| C st m ~> C' st' m' |m>)
+          { struct REACH }
+          : Pm C' st' m').
+  - intros. destruct REACH.
+    + exact INIT.
+    + specialize (MEM C st (e_var x) INIT).
+      destruct st. specialize (MEM (addr_x C x)).
+      inversion STATE; subst. rewrite <- ACCESS in MEM.
+      exact MEM.
+    + apply (IHere C st e1 C' st' e'). eapply APPl.
+      exact INIT. exact REACH.
+    + apply (IHere C st_lam e2 C' st' e').
+      apply APPr with (st := st) (e1 := e1) (C_lam := C_lam) (lam := v).
+      exact INIT. apply (IHere C st e1 C_lam st_lam v).
+      eapply APPl. exact INIT. exact REACH1. exact REACH2.
+    + assert (LAM : Pe C_lam st_lam (e_lam x e)).
+      apply (IHere C st e1 C_lam st_lam (e_lam x e)).
+      eapply APPl. exact INIT. exact REACH1.
+      apply (IHere (C_lam [|dy_c_lam x t dy_c_hole|])
+            (ST (dy_level C_lam ++ [t] !-> Val arg pf C_arg; mem)
+            (update_t t)) e C' st' e').
+      apply APPb with (C := C) (st := st) (e1 := e1) (e2 := e2) (st_lam := st_lam).
+      exact INIT. exact LAM. 
+      apply (IHere C st_lam e2 C_arg (ST mem t) arg).
+      apply (APPr C st e1 e2 C_lam st_lam (e_lam x e)).
+      exact INIT. exact LAM. exact REACH2. exact REACH3.
+    + apply (IHmre C st m C' st' e'). apply LINKm with (e := e). exact INIT. exact REACHm.
+    + apply (IHere C_m st_m e C' st' e'). apply LINKe with (C := C) (st := st) (m := m).
+      exact INIT.
+      apply (IHmrm C st m C_m st_m m_empty).
+      eapply LINKm. exact INIT. exact MODr. exact REACH.
+  - intros. destruct REACH.
+    + apply (IHerm C st e1 C' st' m'). eapply APPl.
+      exact INIT. exact REACH.
+    + apply (IHerm C st_lam e2 C' st' m').
+      eapply APPr with (C_lam := C_lam) (lam := v). exact INIT.
+      apply (IHere C st e1 C_lam st_lam v).
+      eapply APPl. exact INIT. exact FNr. exact REACH.
+    + assert (LAM : Pe C_lam st_lam (e_lam x e)).
+      apply (IHere C st e1 C_lam st_lam (e_lam x e)).
+      eapply APPl. exact INIT. exact FNr.
+      apply (IHerm (C_lam [|dy_c_lam x t dy_c_hole|])
+            (ST (dy_level C_lam ++ [t] !-> Val arg pf C_arg; mem)
+            (update_t t)) e C' st' m').
+      eapply APPb with (st_lam := st_lam). exact INIT. exact LAM.
+      apply (IHere C st_lam e2 C_arg (ST mem t) arg).
+      apply (APPr C st e1 e2 C_lam st_lam (e_lam x e)).
+      exact INIT. exact LAM. exact ARGr. exact REACH.
+    + apply (IHmrm C st m C' st' m').
+      eapply LINKm. exact INIT. exact REACHm.
+    + apply (IHerm C_m st_m e C' st' m').
+      eapply LINKe. exact INIT.
+      apply (IHmrm C st m C_m st_m m_empty).
+      eapply LINKm. exact INIT. exact MODr. exact REACH.
+  - intros. destruct REACH.
+    + apply (IHere C st e C' st' e').
+      eapply LETex. exact INIT. exact REACHe.
+    + apply (IHmre (C [|dy_c_lete x t dy_c_hole|])
+        (ST (dy_level C ++ [t] !-> Val v pf C_x; mem) (update_t t)) m
+        C' st' e').
+      eapply LETem. exact INIT.
+      apply (IHere C st e C_x (ST mem t) v).
+      eapply LETex. exact INIT. exact EVALxr. exact REACH.
+    + apply (IHmre C st m1 C' st' e').
+      eapply LETm1. exact INIT. exact REACH.
+    + apply (IHmre (C [|dy_c_letm M C_M dy_c_hole|]) st_M m2 C' st' e').
+      eapply LETm2. exact INIT.
+      apply (IHmrm C st m1 C_M st_M m_empty).
+      eapply LETm1. exact INIT. exact EVALM0. exact REACH.
+  - intros. destruct REACH.
+    + exact INIT.
+    + specialize (MVAR C st M C_M ACCESS).
+      apply MVAR. exact INIT.
+    + apply (IHerm C st e C' st' m').
+      eapply LETex. exact INIT. exact REACHe.
+    + apply (IHmrm (C [|dy_c_lete x t dy_c_hole|])
+        (ST (dy_level C ++ [t] !-> Val v pf C_x; mem) (update_t t)) m
+        C' st' m').
+      eapply LETem. exact INIT.
+      apply (IHere C st e C_x (ST mem t) v).
+      eapply LETex. exact INIT. exact EVALxr. exact REACH.
+    + apply (IHmrm C st m1 C' st' m').
+      eapply LETm1. exact INIT. exact REACH.
+    + apply (IHmrm (C [|dy_c_letm M C_M dy_c_hole|]) st_M m2 C' st' m').
+      eapply LETm2. exact INIT.
+      apply (IHmrm C st m1 C_M st_M m_empty).
+      eapply LETm1. exact INIT. exact REACH1. exact REACH2.
+Qed.
+
+Definition level_bound ub st :=
     match st with
-    | ST e_mem m_mem t =>
-        (forall (addr : path) v pf p' C',
-                e_mem addr = Some (Val v pf p' C') ->
-                len_p p' + m = level C' + n) /\
-        (forall (addr : path) p' C',
-                m_mem addr = Some (Mod p' C') ->
-                len_p p' + m = level C' + n) /\
-        len_p p + m = level C + n
+    | ST mem _ =>
+        (forall (addr : path),
+          match mem addr with
+          | Some (Val v _ C_v) => level_expr (dy_to_st C_v) v <= ub
+          | None => True
+          end)
     end.
 
-Lemma ere_p_is_level : 
-    forall m n
-           pi Ci sti ei
-           pr Cr str er
-          (INIT : st_len m n pi Ci sti)
-          (REACH : <e| pi Ci sti ei ~> pr Cr str er |e>),
-          st_len m n pr Cr str.
+Lemma ere_level_bound : 
+    forall ub
+           C st e
+           C' st' e'
+          (INIT : level_bound ub st /\ level_expr (dy_to_st C) e <= ub)
+          (REACH : <e| C st e ~> C' st' e' |e>),
+          level_bound ub st' /\ level_expr (dy_to_st C') e' <= ub.
 Proof. 
-  intros m n.
-  apply EreachE_ind_mut with (P := st_len m n).
-  - unfold st_len in *. intros. destruct st. intros.
-    inversion H as [ECASE [MCASE EQ]]. split.
-    + remember (e_mem addr) as e_val.
-      destruct e_val. destruct e. split.
-      intros. eapply ECASE; eauto. split.
-      intros. eapply MCASE; eauto. eapply ECASE; eauto. eauto.
-    + remember (m_mem addr) as m_val.
-      destruct m_val. destruct m0. split.
-      intros. eapply ECASE; eauto. split.
-      intros. eapply MCASE; eauto. eapply MCASE; eauto. eauto.
-  - intros p C st p' C' st' INIT REACH.
-    unfold st_len in *. destruct st, st'. intros.
-    inversion INIT as [ECASEI [MCASEI EQI]].
-    inversion REACH as [ECASER [MCASER EQR]]. split; intros; eauto.
-  - intros. unfold st_len in *.
-    destruct st, st_lam.
-    inversion INIT as [ECASEI [MCASEI EQI]].
-    inversion FN as [ECASEF [MCASEF EQF]].
-    inversion ARG as [ECASEA [MCASEA EQA]].
-    repeat split;
-    intros; unfold update_m in *; try destruct (eq_p addr (t :: p_lam)); eauto.
-    + inversion H; subst; eauto.
-    + rewrite c_plugin_adds_level; simpl. nia.
-  - intros. unfold st_len in *.
-    destruct st.
-    inversion INIT as [ECASEI [MCASEI EQI]].
-    inversion EVx as [ECASEx [MCASEx EQx]].
-    repeat split;
-    intros; unfold update_m in *; try destruct (eq_p addr (t :: p)); eauto.
-    + inversion H; subst; eauto.
-    + rewrite c_plugin_adds_level; simpl. nia.
-  - intros. unfold st_len in *.
-    destruct st.
-    inversion INIT as [ECASEI [MCASEI EQI]].
-    inversion EVM as [ECASEM [MCASEM EQM]].
-    repeat split;
-    intros; unfold update_m in *; try destruct (eq_p addr (t :: p)); eauto.
-    + inversion H; subst; eauto.
-    + rewrite c_plugin_adds_level; simpl. nia.
-Qed.
-
-Lemma preserve_st_len : forall e p' C' st' e'
-        (REACH : <e| [] c_hole (ST empty_mem empty_mem 0) e ~> p' C' st' e' |e>),
-        st_len 0 0 p' C' st'.
-Proof.
-  intros. unfold st_len in *.
-  assert (INIT : st_len 0 0 [] c_hole (ST empty_mem empty_mem 0)).
-  { unfold st_len in *; repeat split; intros; try inversion H. }
-  specialize (ere_p_is_level 0 0 [] c_hole (ST empty_mem empty_mem 0) e
-                             p' C' st' e'
-                             INIT REACH).
-  destruct st'. unfold st_len. eauto.
-Qed.
-
-Theorem level_is_len_p : forall e p' C' st' e'
-        (REACH : <e| [] c_hole (ST empty_mem empty_mem 0) e ~> p' C' st' e' |e>),
-        level C' = len_p p'.
-Proof.
-  pose proof preserve_st_len as H.
-  intros. specialize (H e p' C' st' e' REACH).
-  unfold st_len in H. destruct st'.
-  destruct H as [mem_e [mem_m eq]].
-  nia.
-Qed.
+  intros ub.
+  apply (EreachE_ind_mut
+    (fun C st e =>
+          level_bound ub st /\ 
+          level_expr (dy_to_st C) e <= ub)
+    (fun C st m => 
+          level_bound ub st /\ 
+          let (o, l) := level_mod (dy_to_st C) m in l <= ub)).
+  Admitted.
